L40->L50 stmt

Config.v
@@ -7,7 +7,7 @@ Class VyperConfig := {
   string_set_impl: FSet.class String.string_dec string_set;
   string_map: Type -> Type;
   string_map_impl: forall t: Type, Map.class String.string_dec t (string_map t);
-  world_state: Type;
+  world_state: Type; (* includes memory *)
   uint256: Type;
   Z_of_uint256: uint256 -> Z;
   uint256_of_Z: Z -> uint256;
@@ -18,6 +18,9 @@ Class VyperConfig := {
   memory: Type;
   memory_impl: OpenArray.class (uint256_of_Z 0%Z) memory;
   string_hash: string -> uint256;
+  mload: world_state -> uint256 -> uint256;
+  world_except_memory: Type;
+  get_world_except_memory: world_state -> world_except_memory;
 }.
 
 Lemma two_to_256_ne_0: (2^256 <> 0)%Z.
@@ -39,17 +42,21 @@ Definition sample_config
       string_set_impl := FSet.string_avl_set_impl;
       string_map := Map.string_avl_map;
       string_map_impl := Map.string_avl_map_impl;
-      world_state := Map.string_avl_map Z;
+      world_state := Map.string_avl_map Z * list Z;
       uint256 := Z;
       Z_of_uint256 u := (u mod 2^256)%Z;
       uint256_of_Z z := (z mod 2^256)%Z;
       uint256_ok z := Z.mod_mod _ _ two_to_256_ne_0;
       uint256_range u := Z.mod_pos_bound _ _ two_to_256_pos;
-      storage_lookup := let _ := Map.string_avl_map_impl in Map.lookup;
-      storage_insert := let _ := Map.string_avl_map_impl in Map.insert;
+      storage_lookup w := let _ := Map.string_avl_map_impl in Map.lookup (fst w);
+      storage_insert w key val := (let _ := Map.string_avl_map_impl in Map.insert (fst w) key val,
+                                   snd w);
       memory := list Z;
       memory_impl := OpenArray.list_inst 0%Z;
       string_hash := fun s => (Z.of_N (keccak_256_N_of_string s))%Z;
+      mload w addr := List.nth (Z.to_nat (addr mod 2^256)) (snd w) 0%Z;
+      world_except_memory := Map.string_avl_map Z;
+      get_world_except_memory := fst
    |}.
 
 Definition zero256 {C: VyperConfig} := uint256_of_Z 0%Z.
