From40To50/Proto.v
@@ -1,8 +1,9 @@
-From Coq Require Import String.
+From Coq Require Import Arith NArith String ProofIrrelevance.
 
 From Vyper.L10 Require Import Base.
 From Vyper.L50 Require Import Types Builtins.
-From Vyper Require Import Config ProtoAST NaryFun.
+From Vyper.CheckArith Require Import Builtins.
+From Vyper Require Import Config ProtoAST NaryFun Logic2.
 
 Local Open Scope list_scope.
 Local Open Scope string_scope.
@@ -93,6 +94,216 @@ Definition call_builtin_u256 {C: VyperConfig}
                              (LenOk: List.length (b_input_types b) = List.length args)
 : world_state * expr_result (list uint256)
 := fst (nary_call (b_fun b world) args (PeanoNat.Nat.eq_le_incl _ _ LenOk)).
+
+Definition check_proto (mb_p: option proto) (n_ins n_outs: nat)
+:= match mb_p with
+   | None => false
+   | Some p => (   proto_is_u256_only p
+                && (List.length (p_inputs p)  =? n_ins)
+                && (List.length (p_outputs p) =? n_outs))%bool%nat
+   end.
+
+Definition check_known_protos {C: VyperConfig}
+                              (B: builtin_names_config)
+                              (protos: string -> option proto)
+: bool
+:= check_proto (protos (builtin_name_uint256_add B)) 2 1
+&& check_proto (protos (builtin_name_uint256_sub B)) 2 1
+&& check_proto (protos (builtin_name_uint256_mul B)) 2 1
+&& check_proto (protos (builtin_name_uint256_div B)) 2 1
+&& check_proto (protos (builtin_name_uint256_mod B)) 2 1
+&& check_proto (protos (builtin_name_uint256_pow B)) 2 1
+&& check_proto (protos (builtin_name_uint256_not B)) 1 1
+&& check_proto (protos (builtin_name_uint256_iszero B)) 1 1
+&& check_proto (protos (builtin_name_uint256_and B)) 2 1
+&& check_proto (protos (builtin_name_uint256_or B))  2 1
+&& check_proto (protos (builtin_name_uint256_xor B)) 2 1
+&& check_proto (protos (builtin_name_uint256_lt B))  2 1
+&& check_proto (protos (builtin_name_uint256_eq B))  2 1
+&& check_proto (protos (builtin_name_uint256_shl B)) 2 1
+&& check_proto (protos (builtin_name_uint256_shr B)) 2 1
+&& check_proto (protos "mstore") 2 0
+&& check_proto (protos "revert") 2 0
+&& check_proto (protos "stop") 0 0
+&& check_proto (protos "pop") 1 0
+&& check_proto (protos "sload") 1 1
+&& check_proto (protos "sstore") 2 0.
+
+
+(** Value agreement between L40 and L50.
+    [n]: expected length of [e50]
+    The tricky part here is that L50 might have no value where L40 sees zero. 
+ *)
+Definition ExprResultsAgree {C: VyperConfig}
+                            (e40: expr_result uint256)
+                            (e50: expr_result (list dynamic_value))
+                            (n: N)
+:= match e40, e50 with
+   | ExprAbort a40, ExprAbort a50               =>  a40 = a50
+   | ExprSuccess v40, ExprSuccess nil           =>  v40 = zero256 %Z /\ n = 0%N
+   | ExprSuccess v40, ExprSuccess (v50 :: nil)  =>  (* v40 = uint256_of_dynamic_value v50 *)
+                                                    v50 = (existT _ U256 (yul_uint256 v40)) /\ n = 1%N
+   | _, _ => False
+   end.
+
+
+(** Value agreement between L40 and L50, a variant with u256 list on the L50 side.
+    [n]: expected length of [e50]
+    The tricky part here is that L50 might have no value where L40 sees zero.
+ *)
+Definition ExprResultsAgree256 {C: VyperConfig}
+                               (e40: expr_result uint256)
+                               (e50: expr_result (list uint256))
+                               (n: N)
+:= match e40, e50 with
+   | ExprAbort a40, ExprAbort a50               =>  a40 = a50
+   | ExprSuccess v40, ExprSuccess nil           =>  v40 = zero256%Z /\ n = 0%N
+   | ExprSuccess v40, ExprSuccess (v50 :: nil)  =>  v40 = v50 /\ n = 1%N
+   | _, _ => False
+   end.
+
+
+Definition BuiltinsAgree {C: VyperConfig}
+                         (b40: builtin)
+                         (b50: L50.Builtins.yul_builtin)
+                         (B50InputsU256:   L50.Builtins.all_are_u256 (L50.Builtins.b_input_types  b50) = true)
+                         (B50OutputssU256: L50.Builtins.all_are_u256 (L50.Builtins.b_output_types b50) = true)
+:= let '(existT _ arity f40) := b40 in
+       arity = List.length (L50.Builtins.b_input_types b50)
+        /\
+       forall (world: world_state) (args: list uint256)
+              (LenOk40: (arity =? List.length args = true)%nat)
+              (LenOk50: List.length (Builtins.b_input_types b50) = List.length args),
+         let (w40, e40) := (L10.Base.call_builtin args LenOk40 (f40 world)) in
+         let (w50, e50) := (call_builtin_u256 b50 world args LenOk50) in
+         w40 = w50  /\  ExprResultsAgree256 e40 e50 
+                                            (N.of_nat (List.length (L50.Builtins.b_output_types b50))).
+
+Definition AllBuiltinsAgreeIfU256 {C: VyperConfig}
+                                  (builtins40: string -> option builtin)
+                                  (builtins50: string -> option L50.Builtins.yul_builtin)
+:= forall name: string,
+     match builtins50 name with
+     | None => True
+     | Some b50 =>
+        (if L50.Builtins.all_are_u256 (L50.Builtins.b_input_types b50) as z return _ = z -> _
+         then 
+           fun i256 =>
+            (if L50.Builtins.all_are_u256 (L50.Builtins.b_output_types b50) as z return _ = z -> _
+              then fun o256 =>
+                   match builtins40 name with
+                   | None => False
+                   | Some b40 => BuiltinsAgree b40 b50 i256 o256
+                   end
+              else fun _ => True) eq_refl
+         else fun _ => True) eq_refl
+     end.
+
+Lemma binop_to_yul {C: VyperConfig}
+                   {builtins40: string -> option L10.Base.builtin}
+                   {builtins50: string -> option L50.Builtins.yul_builtin}
+                   (BuiltinsOk: AllBuiltinsAgreeIfU256 builtins40 builtins50)
+                   {protos: string -> option proto}
+                   (ProtosOk: ProtosAgree protos builtins50)
+                   {name: string}
+                   (ProtoOk: check_proto (protos name) 2 1 = true)
+                   {binop: uint256 -> uint256 -> uint256}
+                   (Support40: BuiltinsSupportBinop builtins40 name binop):
+  match builtins50 name with
+  | Some b => forall w x y,
+                L50.Builtins.call_builtin b w 
+                     (existT _ U256 (yul_uint256 x) :: existT _ U256 (yul_uint256 y) :: nil)
+                 =
+                (w, ExprSuccess (existT _ U256 (yul_uint256 (binop x y)) :: nil))
+  | None => False
+  end.
+Proof.
+assert (P := ProtosOk name).
+unfold check_proto in ProtoOk.
+destruct (protos name) as [p|]. 2:discriminate.
+assert (A := BuiltinsOk name).
+destruct (builtins50 name) as [b|]. 2:contradiction.
+destruct P as (InputsAgree, OutputsAgree).
+(* we have:
+  InputsAgree : p_inputs p = b_input_types b
+  OutputsAgree : p_outputs p = b_output_types b
+*)
+unfold proto_is_u256_only in ProtoOk.
+apply andb_prop in ProtoOk. destruct ProtoOk as (ProtoOk, OutputLenIs1).
+apply andb_prop in ProtoOk. destruct ProtoOk as (ProtoOk, InputLenIs2).
+apply andb_prop in ProtoOk. destruct ProtoOk as (InputsAreU256, OutputsAreU256).
+rewrite InputsAgree in InputsAreU256. rewrite OutputsAgree in OutputsAreU256.
+rewrite InputsAgree in InputLenIs2. rewrite OutputsAgree in OutputLenIs1.
+apply Nat.eqb_eq in InputLenIs2. apply Nat.eqb_eq in OutputLenIs1.
+rewrite if_yes with (E := InputsAreU256) in A.
+rewrite if_yes with (E := OutputsAreU256) in A.
+unfold BuiltinsSupportBinop in Support40.
+destruct (builtins40 name) as [(arity40, f40)|]. 2:contradiction.
+unfold BuiltinsAgree in A.
+unfold BuiltinIsBinop in Support40. cbn in Support40.
+destruct arity40. { destruct A as (A, _). now rewrite InputLenIs2 in A. }
+destruct arity40. { destruct A as (A, _). now rewrite InputLenIs2 in A. }
+destruct arity40. 2:{ destruct A as (A, _). now rewrite InputLenIs2 in A. }
+destruct A as (_, A).
+unfold L10.Base.call_builtin in A.
+intros w x y.
+assert (LenOk50: Datatypes.length (b_input_types b) = Datatypes.length (x :: y :: nil))
+  by apply InputLenIs2.
+assert (V := A w (x :: y :: nil) eq_refl LenOk50).
+cbn in V. clear A.
+cbn in Support40. rewrite Support40 in V.
+rewrite OutputLenIs1 in V. cbn in V.
+assert (BI: b_input_types b = U256 :: U256 :: nil).
+{
+  clear V.
+  remember (b_input_types b) as z.
+  destruct z as [|u]. { easy. }
+  destruct z as [|v]. { easy. }
+  destruct z. 2:easy.
+  cbn in InputsAreU256.
+  destruct (yul_type_eq_dec u U256) as [Eu|NE]. 2:easy.
+  destruct (yul_type_eq_dec v U256) as [Ev|NE]. 2:easy.
+  now subst u v.
+}
+unfold call_builtin.
+assert (TypecheckOk: mass_typecheck
+                      (existT (fun t : yul_type => yul_value t) U256 (yul_uint256 x)
+                       :: existT (fun t : yul_type => yul_value t) U256 (yul_uint256 y) :: nil) 
+                      (b_input_types b) = MassTypecheckOk)
+  by now rewrite BI.
+rewrite mass_typecheck_ok_rewrite with (Ok := TypecheckOk).
+unfold call_builtin_u256 in V.
+cbn.
+remember ((Nat.eq_le_incl (Datatypes.length (b_input_types b)) (Datatypes.length (x :: y :: nil))
+              LenOk50)) as foo.
+remember ((Builtins.call_builtin_helper b
+        (existT (fun t : yul_type => yul_value t) U256 (yul_uint256 x)
+         :: existT (fun t : yul_type => yul_value t) U256 (yul_uint256 y) :: nil) TypecheckOk))
+  as bar.
+clear Heqfoo. clear Heqbar.
+assert (foo = bar) by apply proof_irrelevance. subst bar.
+destruct (nary_call (b_fun b w) (x :: y :: nil) foo) as ((w50, r50), trash).
+cbn in V. destruct V as (W, V). subst w50.
+destruct r50 as [result|]. 2:easy.
+assert (BO: b_output_types b = U256 :: nil).
+{
+  clear V.
+  remember (b_output_types b) as z.
+  destruct z as [|u]. { easy. }
+  destruct z. 2:easy.
+  cbn in OutputsAreU256.
+  destruct (yul_type_eq_dec u U256) as [Eu|NE]. 2:easy.
+  now subst u.
+}
+rewrite BO.
+destruct result. 1:easy.
+destruct result. 2:easy.
+destruct V as (V, _).
+subst u.
+unfold mass_cast.
+now rewrite yul_value_of_uint256_u256.
+Qed.
+
 
 
 (*
