L50/Stmt.v
@@ -1,6 +1,6 @@
 From Coq Require Import String Arith ZArith.
 
-From Vyper Require Import Config Map.
+From Vyper Require Import Config Map Logic2.
 From Vyper.L10 Require Import Base.
 From Vyper.L50 Require Import Types AST Builtins Expr LocalVars DynError.
 
@@ -61,12 +61,20 @@ Fixpoint interpret_stmt {C: VyperConfig}
    | If cond yes => fun _ =>
            match interpret_expr builtins funs do_call world loc cond
            with
+           (* Apparently the actual Yul does not require boolean conditions in if and for.
            | (world', Some (ExprSuccess (existT _ BoolType (BoolValue _ b _) :: nil))) =>
                if b
                  then interpret_block max_loop_iterations
                                       builtins funs this_fun_decl do_call
-                                      world loc nop yes
+                                      world' loc nop yes
                  else (world', loc, Some StmtSuccess)
+           *)
+           | (world', Some (ExprSuccess (b :: nil))) =>
+               if (Z_of_uint256 (uint256_of_dynamic_value b) =? 0)%Z
+                 then (world', loc, Some StmtSuccess)
+                 else interpret_block max_loop_iterations
+                                      builtins funs this_fun_decl do_call
+                                      world' loc nop yes
            | (world', Some (ExprSuccess _)) =>
                 (world', loc, Some (stmt_error (string_of_dynamic_error DE_SingleBooleanExpected)))
            | (world', Some (ExprAbort ab)) => (world', loc, Some (StmtAbort ab))
@@ -95,7 +103,7 @@ Fixpoint interpret_stmt {C: VyperConfig}
                                  Z_of_uint256 (uint256_of_yul_value guard))%Z
                                 then interpret_block max_loop_iterations
                                                      builtins funs this_fun_decl do_call
-                                                     world loc nop body
+                                                     world' loc nop body
                                 else dispatch tail
                         else (world', loc, Some (stmt_error (string_of_dynamic_error
                                                               (DE_TypeMismatch guard_type value_type))))
@@ -104,7 +112,7 @@ Fixpoint interpret_stmt {C: VyperConfig}
                            | Some body =>
                                 interpret_block max_loop_iterations
                                                 builtins funs this_fun_decl do_call
-                                                world loc nop body
+                                                world' loc nop body
                            | None => (world', loc, Some StmtSuccess)
                            end
                   end) cases
@@ -121,9 +129,13 @@ Fixpoint interpret_stmt {C: VyperConfig}
                | S count' =>
                    match interpret_expr builtins funs do_call world loc cond
                    with
-                   | (world', Some (ExprSuccess (existT _ BoolType (BoolValue _ b _) :: nil))) =>
-                       if b
-                         then match interpret_block max_loop_iterations
+                   (* as in If, I removed the check that the condition is actually a boolean
+                      because the actual implementation never enforces that.
+                    *)
+                   | (world', Some (ExprSuccess (b :: nil))) =>
+                       if (Z_of_uint256 (uint256_of_dynamic_value b) =? 0)%Z
+                         then (world', loc, Some StmtSuccess)
+                         else match interpret_block max_loop_iterations
                                                     builtins funs this_fun_decl do_call
                                                     world' loc nop body
                               with
@@ -146,7 +158,6 @@ Fixpoint interpret_stmt {C: VyperConfig}
                                   end
                               | x => x
                               end
-                         else (world', loc, Some StmtSuccess)
                    | (world', Some (ExprSuccess _)) =>
                         (world', loc, Some (stmt_error (string_of_dynamic_error DE_SingleBooleanExpected)))
                    | (world', Some (ExprAbort ab)) => (world', loc, Some (StmtAbort ab))
@@ -218,3 +229,367 @@ with interpret_block {C: VyperConfig}
                       end) eq_refl
            end eq_refl
     in let '(Block stmts) := b in interpret_stmt_list world loc stmts.
+
+(** In all cases except for-loops' init blocks we don't need the stupid postproc hook.
+  Here's a cleaner hook-free version.
+ *)
+Fixpoint interpret_stmt_list {C: VyperConfig}
+                             (max_loop_iterations: nat)
+                             (builtins: string -> option yul_builtin)
+                             (funs: string -> option fun_decl)
+                             (this_fun_decl: option fun_decl)
+                             (do_call: fun_decl -> world_state -> list dynamic_value ->
+                                         world_state * option (expr_result (list dynamic_value)))
+                             (world: world_state)
+                             (loc: string_map dynamic_value)
+                             (stmts: list stmt)
+{struct stmts}
+: world_state * string_map dynamic_value * option (stmt_result (list dynamic_value))
+:= match stmts as stmts' return stmts = stmts' -> _ with
+   | nil => fun _ => (world, loc, Some StmtSuccess)
+   | h :: t => fun E =>
+      (if is_var_decl h as h_is_var_decl return _ = h_is_var_decl -> _
+         then fun Evar =>
+           match var_decl_unpack h Evar with
+           | (names, Some init) =>
+                match interpret_expr builtins funs do_call world loc init
+                with
+                | (world', Some (ExprSuccess values)) =>
+                    match bind_vars_to_values names values loc with
+                    | inl err => (world', loc, Some (stmt_error (string_of_dynamic_error err)))
+                    | inr loc' =>
+                        let '(world'', loc'', result) := 
+                            interpret_stmt_list max_loop_iterations builtins funs this_fun_decl do_call
+                                                world' loc' t in
+                        (world'', unbind_vars names loc'', result)
+                    end
+                | (world', Some (ExprAbort ab)) => (world', loc, Some (StmtAbort ab))
+                | (world', None) => (world', loc, None)
+                end
+           | (names, None) =>
+               match bind_vars_to_zeros names loc with
+               | inl err => (world, loc, Some (stmt_error (string_of_dynamic_error err)))
+               | inr loc' =>
+                   let '(world', loc'', result) := interpret_stmt_list max_loop_iterations builtins
+                                                                       funs this_fun_decl do_call
+                                                                       world loc' t 
+                   in (world', unbind_vars names loc'', result)
+               end
+           end
+         else fun Evar =>
+           let '(world', loc', result) := interpret_stmt max_loop_iterations
+                                                         builtins funs this_fun_decl do_call
+                                                         world loc h Evar
+           in match result with
+              | Some StmtSuccess => interpret_stmt_list max_loop_iterations builtins
+                                                        funs this_fun_decl do_call
+                                                        world' loc' t
+              | _ => (world', loc', result)
+              end) eq_refl
+   end eq_refl.
+
+(** The standalone definition of [interpret_stmt_list] corresponds to interpret_block. *)
+Lemma interpret_stmt_list_ok {C: VyperConfig}
+                             (max_loop_iterations: nat)
+                             (builtins: string -> option yul_builtin)
+                             (funs: string -> option fun_decl)
+                             (this_fun_decl: option fun_decl)
+                             (do_call: fun_decl -> world_state -> list dynamic_value ->
+                                         world_state * option (expr_result (list dynamic_value)))
+                             (world: world_state)
+                             (loc: string_map dynamic_value)
+                             (stmts: list stmt):
+  interpret_block max_loop_iterations builtins funs this_fun_decl do_call world loc nop (Block stmts)
+   =
+  interpret_stmt_list max_loop_iterations builtins funs this_fun_decl do_call world loc stmts.
+Proof.
+cbn. (* open interpret_block *)
+revert world loc. induction stmts as [|head]; intros. { easy. }
+cbn.
+pose (x := is_var_decl head). remember x as head_is_var_decl. symmetry in Heqhead_is_var_decl.
+destruct head_is_var_decl; subst x.
+{
+  repeat rewrite if_yes with (E := Heqhead_is_var_decl).
+  destruct (var_decl_unpack head Heqhead_is_var_decl) as (names, inits).
+  destruct inits as [inits|].
+  {
+    destruct (interpret_expr builtins funs do_call world loc inits) as (world', init_result).
+    destruct init_result as [init_result|]. 2:easy.
+    destruct init_result as [values|ab]. 2:easy.
+    destruct (bind_vars_to_values names values loc). { easy. }
+    rewrite IHstmts. trivial.
+  }
+  destruct (bind_vars_to_zeros names loc). { easy. }
+  rewrite IHstmts. trivial.
+}
+repeat rewrite if_no with (E := Heqhead_is_var_decl).
+destruct interpret_stmt as ((world', loc'), head_result).
+destruct head_result as [head_result|]. 2:trivial.
+now destruct head_result.
+Qed.
+
+(** This version of [interpret_stmt_list] doesn't unbind the declared local variables,
+    instead it returns a list of them.
+    This is necessary to reason about interpreting a list of the form [a ++ b].
+ *)
+Fixpoint interpret_stmt_list_no_unbind {C: VyperConfig}
+                                       (max_loop_iterations: nat)
+                                       (builtins: string -> option yul_builtin)
+                                       (funs: string -> option fun_decl)
+                                       (this_fun_decl: option fun_decl)
+                                       (do_call: fun_decl -> world_state -> list dynamic_value ->
+                                                   world_state * option (expr_result (list dynamic_value)))
+                                       (world: world_state)
+                                       (loc: string_map dynamic_value)
+                                       (stmts: list stmt)
+{struct stmts}
+: world_state * string_map dynamic_value * option (stmt_result (list dynamic_value)) * list typename
+:= match stmts as stmts' return stmts = stmts' -> _ with
+   | nil => fun _ => (world, loc, Some StmtSuccess, nil)
+   | h :: t => fun E =>
+      (if is_var_decl h as h_is_var_decl return _ = h_is_var_decl -> _
+         then fun Evar =>
+           match var_decl_unpack h Evar with
+           | (names, Some init) =>
+                match interpret_expr builtins funs do_call world loc init
+                with
+                | (world', Some (ExprSuccess values)) =>
+                    match bind_vars_to_values names values loc with
+                    | inl err => (world', loc, Some (stmt_error (string_of_dynamic_error err)), nil)
+                    | inr loc' =>
+                        let '(world'', loc'', result, vars) :=
+                            interpret_stmt_list_no_unbind max_loop_iterations builtins
+                                                          funs this_fun_decl do_call
+                                                          world' loc' t
+                        in (world'', loc'', result, vars ++ names)
+                    end
+                | (world', Some (ExprAbort ab)) => (world', loc, Some (StmtAbort ab), nil)
+                | (world', None) => (world', loc, None, nil)
+                end
+           | (names, None) =>
+               match bind_vars_to_zeros names loc with
+               | inl err => (world, loc, Some (stmt_error (string_of_dynamic_error err)), nil)
+               | inr loc' =>
+                   let '(world', loc'', result, vars) :=
+                            interpret_stmt_list_no_unbind max_loop_iterations builtins
+                                                          funs this_fun_decl do_call
+                                                          world loc' t
+                   in (world', loc'', result, vars ++ names)
+               end
+           end
+         else fun Evar =>
+           let '(world', loc', result) := interpret_stmt max_loop_iterations
+                                                         builtins funs this_fun_decl do_call
+                                                         world loc h Evar
+           in match result with
+              | Some StmtSuccess => interpret_stmt_list_no_unbind max_loop_iterations builtins
+                                                                  funs this_fun_decl do_call
+                                                                  world' loc' t
+              | _ => (world', loc', result, nil)
+              end) eq_refl
+   end eq_refl.
+
+(** [interpret_stmt_list_no_unbind] followed by [unbind_vars] does the same thing
+    as [interpret_stmt_list].
+ *)
+Lemma interpret_stmt_list_unbind_later {C: VyperConfig}
+                                       (max_loop_iterations: nat)
+                                       (builtins: string -> option yul_builtin)
+                                       (funs: string -> option fun_decl)
+                                       (this_fun_decl: option fun_decl)
+                                       (do_call: fun_decl -> world_state -> list dynamic_value ->
+                                                   world_state * option (expr_result (list dynamic_value)))
+                                       (world: world_state)
+                                       (loc: string_map dynamic_value)
+                                       (stmts: list stmt):
+  interpret_stmt_list max_loop_iterations builtins funs this_fun_decl do_call world loc stmts
+   =
+  let '(world', loc', result, vars) :=
+    interpret_stmt_list_no_unbind max_loop_iterations builtins funs this_fun_decl do_call
+                                  world loc stmts
+  in (world', unbind_vars vars loc', result).
+Proof.
+revert world loc. induction stmts as [|head]; intros. { easy. }
+cbn.
+pose (x := is_var_decl head). remember x as head_is_var_decl. symmetry in Heqhead_is_var_decl.
+destruct head_is_var_decl; subst x.
+{
+  repeat rewrite if_yes with (E := Heqhead_is_var_decl).
+  destruct (var_decl_unpack head Heqhead_is_var_decl) as (names, inits).
+  destruct inits as [inits|].
+  {
+    destruct (interpret_expr builtins funs do_call world loc inits) as (world', init_result).
+    destruct init_result as [init_result|]. 2:easy.
+    destruct init_result as [values|ab]. 2:easy.
+    destruct (bind_vars_to_values names values loc). { easy. }
+    rewrite IHstmts.
+    destruct interpret_stmt_list_no_unbind as (((w, l), r), v).
+    rewrite unbind_vars_app. trivial.
+  }
+  destruct (bind_vars_to_zeros names loc). { easy. }
+  rewrite IHstmts.
+  destruct interpret_stmt_list_no_unbind as (((w, l), r), v).
+  rewrite unbind_vars_app. trivial.
+}
+repeat rewrite if_no with (E := Heqhead_is_var_decl).
+destruct interpret_stmt as ((world', loc'), head_result).
+destruct head_result as [head_result|]. 2:trivial.
+now destruct head_result.
+Qed.
+
+(** Interpreting [a ++ b].
+    (This lemma is the reason for interpret_stmt_list_no_unbind).
+ *)
+Lemma interpret_stmt_list_no_unbind_app {C: VyperConfig}
+                                        (max_loop_iterations: nat)
+                                        (builtins: string -> option yul_builtin)
+                                        (funs: string -> option fun_decl)
+                                        (this_fun_decl: option fun_decl)
+                                        (do_call: fun_decl -> world_state -> list dynamic_value ->
+                                                    world_state * option (expr_result (list dynamic_value)))
+                                        (world: world_state)
+                                        (loc: string_map dynamic_value)
+                                        (a b: list stmt):
+  interpret_stmt_list_no_unbind max_loop_iterations builtins funs this_fun_decl do_call
+                                world loc (a ++ b)
+   =
+  let '(world', loc', result', vars') :=
+    interpret_stmt_list_no_unbind max_loop_iterations builtins funs this_fun_decl do_call
+                                  world loc a
+  in match result' with
+     | Some StmtSuccess =>
+        let '(world'', loc'', result'', vars'') :=
+             interpret_stmt_list_no_unbind max_loop_iterations builtins funs this_fun_decl do_call
+                                           world' loc' b
+        in (world'', loc'', result'', vars'' ++ vars')
+     | _ => (world', loc', result', vars')
+     end.
+Proof.
+revert world loc. induction a as [|head]; intros.
+{
+  rewrite List.app_nil_l. cbn.
+  destruct interpret_stmt_list_no_unbind as (((w, l), r), v).
+  now rewrite List.app_nil_r.
+}
+cbn.
+pose (x := is_var_decl head). remember x as head_is_var_decl. symmetry in Heqhead_is_var_decl.
+destruct head_is_var_decl; subst x.
+{
+  repeat rewrite if_yes with (E := Heqhead_is_var_decl).
+  destruct (var_decl_unpack head Heqhead_is_var_decl) as (names, inits).
+  destruct inits as [inits|].
+  {
+    destruct (interpret_expr builtins funs do_call world loc inits) as (world', init_result).
+    destruct init_result as [init_result|]. 2:easy.
+    destruct init_result as [values|ab]. 2:easy.
+    destruct (bind_vars_to_values names values loc). { easy. }
+    rewrite IHa.
+    destruct interpret_stmt_list_no_unbind as (((w, l), r), v).
+    destruct r as [r|]. 2:easy. destruct r; try easy.
+    destruct interpret_stmt_list_no_unbind as (((w', l'), r'), v').
+    now rewrite List.app_assoc.
+  }
+  destruct (bind_vars_to_zeros). { easy. }
+  rewrite IHa.
+  destruct interpret_stmt_list_no_unbind as (((w, l), r), v).
+  destruct r as [r|]. 2:easy. destruct r; try easy.
+  destruct interpret_stmt_list_no_unbind as (((w', l'), r'), v').
+  now rewrite List.app_assoc.
+}
+repeat rewrite if_no with (E := Heqhead_is_var_decl).
+destruct interpret_stmt as ((w, l), r).
+destruct r as [r|]. 2:easy. now destruct r.
+Qed.
+
+Fixpoint stmt_list_has_top_level_var_decls {C: VyperConfig}
+                                           (l: list stmt)
+:= match l with
+   | nil => false
+   | h :: t => (is_var_decl h  ||  stmt_list_has_top_level_var_decls t)%bool
+   end.
+
+Lemma stmt_list_has_top_level_var_decls_app {C: VyperConfig}
+                                            (a b: list L50.AST.stmt):
+   stmt_list_has_top_level_var_decls (a ++ b)
+    =
+   (stmt_list_has_top_level_var_decls a ||
+    stmt_list_has_top_level_var_decls b)%bool.
+Proof.
+induction a as [|ha]. { easy. }
+cbn.
+rewrite<- Bool.orb_assoc. f_equal.
+assumption.
+Qed.
+
+Lemma interpret_stmt_list_no_unbind_no_vars
+                                       {C: VyperConfig}
+                                       (max_loop_iterations: nat)
+                                       (builtins: string -> option yul_builtin)
+                                       (funs: string -> option fun_decl)
+                                       (this_fun_decl: option fun_decl)
+                                       (do_call: fun_decl -> world_state -> list dynamic_value ->
+                                                   world_state * option (expr_result (list dynamic_value)))
+                                       (world: world_state)
+                                       (loc: string_map dynamic_value)
+                                       (stmts: list stmt)
+                                       (NoVars: stmt_list_has_top_level_var_decls stmts = false):
+  let '(_, _, _, vars) := interpret_stmt_list_no_unbind max_loop_iterations builtins funs
+                                                        this_fun_decl do_call
+                                                        world loc stmts
+  in vars = nil.
+Proof.
+revert world loc. induction stmts as [|head]; intros. { easy. }
+cbn in NoVars. apply Bool.orb_false_elim in NoVars. destruct NoVars as (NoVarsHead, NoVarsTail).
+cbn.
+rewrite if_no with (E := NoVarsHead).
+destruct interpret_stmt as ((world', loc'), result).
+destruct result as [result|]. 2:easy.
+destruct result; try easy. apply IHstmts. assumption.
+Qed.
+
+(** Interpreting [a ++ b] when neither [a] nor [b] contain local variable declarations.
+ *)
+Lemma interpret_stmt_list_app {C: VyperConfig}
+                              (max_loop_iterations: nat)
+                              (builtins: string -> option yul_builtin)
+                              (funs: string -> option fun_decl)
+                              (this_fun_decl: option fun_decl)
+                              (do_call: fun_decl -> world_state -> list dynamic_value ->
+                                          world_state * option (expr_result (list dynamic_value)))
+                              (world: world_state)
+                              (loc: string_map dynamic_value)
+                              (a b: list stmt)
+                              (NoVarsA: stmt_list_has_top_level_var_decls a = false)
+                              (NoVarsB: stmt_list_has_top_level_var_decls b = false):
+  interpret_stmt_list max_loop_iterations builtins funs this_fun_decl do_call
+                      world loc (a ++ b)
+   =
+  let '(world', loc', result') :=
+    interpret_stmt_list max_loop_iterations builtins funs this_fun_decl do_call
+                        world loc a
+  in match result' with
+     | Some StmtSuccess =>
+        let '(world'', loc'', result'') :=
+             interpret_stmt_list max_loop_iterations builtins funs this_fun_decl do_call
+                                 world' loc' b
+        in (world'', loc'', result'')
+     | _ => (world', loc', result')
+     end.
+Proof.
+repeat rewrite interpret_stmt_list_unbind_later.
+rewrite interpret_stmt_list_no_unbind_app.
+assert (V_A := interpret_stmt_list_no_unbind_no_vars max_loop_iterations builtins funs
+                                                     this_fun_decl do_call
+                                                     world loc a NoVarsA).
+destruct (interpret_stmt_list_no_unbind max_loop_iterations builtins funs this_fun_decl do_call world loc a)
+  as (((world', loc'), result'), vars'). subst vars'.
+destruct result' as [result'|]; try easy.
+destruct result'; try easy.
+cbn.
+assert (V_B := interpret_stmt_list_no_unbind_no_vars max_loop_iterations builtins funs
+                                                     this_fun_decl do_call
+                                                     world' loc' b NoVarsB).
+rewrite interpret_stmt_list_unbind_later.
+destruct (interpret_stmt_list_no_unbind max_loop_iterations builtins funs this_fun_decl do_call world' loc' b)
+  as (((world'', loc''), result''), vars''). now subst vars''.
+Qed.
