From40To50/Builtins.v
@@ -1,0 +1,49 @@
+From Coq Require Import String NArith ZArith DecimalString List Lia.
+
+From Vyper Require Import Config NaryFun.
+From Vyper.CheckArith Require Import Builtins.
+From Vyper.L10 Require Import Base.
+From Vyper.L40 Require AST.
+From Vyper.L50 Require AST.
+From Vyper.L50 Require Import Types Expr.
+
+From Vyper.L40Metered Require Import Interpret.
+
+From Vyper.From40To50 Require Import Translate Proto.
+
+(* We need to wrap L50 builtins into L40 versions
+   that perform the same typechecks that the L50 interpreter does.
+
+   This is not really necessary with the default list of builtins which is all u256-typed
+   (address is not a Yul type and is not typechecked).
+ *)
+
+(**
+  Typecheck each argument of a [nary_fun].
+  Equivalent to running [L50.Builtins.mass_typecheck] before calling
+  except no length check on input_types is performed.
+ *)
+Fixpoint embed_typechecks {C: VyperConfig}
+                          {arity: nat}
+                          {ReturnType: Type}
+                          (f: NaryFun.nary_fun uint256 arity (world_state * expr_result ReturnType))
+                          (input_types: list yul_type)
+                          (world: world_state)
+: NaryFun.nary_fun uint256 arity (world_state * expr_result ReturnType)
+:= match arity, f with
+   | 0, result  => result
+   | S arity', g =>
+      match input_types with
+      | nil => g
+      | (head_type :: tail_types)%list =>
+          fun arg =>
+            embed_typechecks 
+      end
+   end.
+
+(*
+L10.Base.builtin
+L50.Builtins.yul_builtin
+L10.Base.call_builtin
+L50.Builtins.call_builtin
+*)
