From40To50/Mangle.v
@@ -1,0 +1,141 @@
+From Coq Require Import Ascii String List NArith DecimalString DecimalN DecimalPos.
+
+From Vyper Require Import Config.
+From Vyper.CheckArith Require Import Builtins.
+From Vyper.L10 Require Import Base.
+
+From Vyper.From40To50 Require Import Translate Proto.
+
+
+Definition starts_with_dollar (s: string)
+: bool
+:= match s with
+   | String "$"%char _ => true
+   | _ => false
+   end.
+
+Lemma starts_with_dollar_eqb (head: ascii) (tail: string):
+  starts_with_dollar (String head tail) = Ascii.eqb head "$"%char.
+Proof.
+cbn.
+destruct head as (b0, b1, b2, b3, b4, b5, b6, b7).
+now destruct b0, b1, b2, b3, b4, b5, b6, b7.
+Qed.
+
+(** [translate_fun_decls] prefixes everything with '$'. *)
+Lemma translated_decls_start_with_dollar {C: VyperConfig}
+                                {B: builtin_names_config}
+                                {protos: string_map proto}
+                                (decls40: string_map L40.AST.decl)
+                                (decls50: string_map L50.AST.fun_decl)
+                                (DeclsOk: translate_fun_decls B protos decls40 = inr decls50)
+                                (name: string)
+                                (Ok: map_lookup decls50 name <> None):
+  starts_with_dollar name = true.
+Proof.
+unfold translate_fun_decls in DeclsOk.
+remember (Map.items decls40) as items40. clear Heqitems40.
+revert decls50 DeclsOk Ok.
+induction items40 as [|(k,v)]; intros; cbn in DeclsOk.
+{
+  inversion DeclsOk. subst. unfold map_lookup in Ok.
+  now rewrite Map.empty_lookup in Ok.
+}
+destruct (translate_fun_decl B protos v). { discriminate. }
+destruct alist_maybe_map_kv. { discriminate. }
+cbn in DeclsOk. inversion DeclsOk. subst. clear DeclsOk.
+unfold map_lookup in Ok. rewrite Map.insert_ok in Ok.
+remember (string_dec (String "$" k) name) as found.
+destruct found. { now subst. }
+unfold map_lookup in IHitems40.
+now refine (IHitems40 _ _ Ok).
+Qed.
+
+(** The same as the previous one but more convenient to use for builtins. *)
+Lemma unmangled_names_are_not_translated {C: VyperConfig}
+                                         {B: builtin_names_config}
+                                         {protos: string_map proto}
+                                         (decls40: string_map L40.AST.decl)
+                                         (decls50: string_map L50.AST.fun_decl)
+                                         (DeclsOk: translate_fun_decls B protos decls40 = inr decls50)
+                                         (name: string)
+                                         (Ok: starts_with_dollar name = false):
+  map_lookup decls50 name = None.
+Proof.
+remember (map_lookup decls50 name) as d. destruct d; trivial.
+assert (NE: map_lookup decls50 name <> None). { rewrite<- Heqd. discriminate. }
+rewrite (translated_decls_start_with_dollar decls40 decls50 DeclsOk name NE) in Ok.
+discriminate.
+Qed.
+
+Lemma mangled_safety_equiv {T} (builtins: string -> option T):
+  (forall x, builtins ("$" ++ x)%string = None)
+   <->
+  (forall x, builtins x <> None -> starts_with_dollar x = false).
+Proof.
+cbn.
+split.
+{
+  intros H x Ok.
+  destruct x as [|head]. { easy. }
+  rewrite starts_with_dollar_eqb.
+  cbn.
+  remember ((head =? "$")%char) as head_is_dollar. destruct head_is_dollar. 2:trivial.
+  symmetry in Heqhead_is_dollar. apply Ascii.eqb_eq in Heqhead_is_dollar.
+  subst. exfalso. exact (Ok (H x)).
+}
+intros H x.
+assert (Ok := H (String "$"%char x)). clear H.
+remember (builtins (String "$" x)) as b. destruct b. 2:trivial.
+clear Heqb. cbn in Ok. exfalso. assert (W: Some t <> None) by discriminate.
+assert (Ok' := Ok W). discriminate.
+Qed.
+
+(***************************************************************************************************)
+
+(* not in standard library? oh well *)
+Lemma string_app_l_inj (a b c: string)
+                       (E: (a ++ b = a ++ c)%string):
+  b = c.
+Proof.
+induction a as [|h]. { easy. }
+cbn in E. inversion E. tauto.
+Qed.
+
+(* why is it not in stdlib? *)
+Lemma to_uint_nonnil (a: N):
+  N.to_uint a <> Decimal.Nil.
+Proof.
+destruct a as [|p]. { easy. }
+cbn. apply Unsigned.to_uint_nonnil.
+Qed.
+
+Lemma string_of_N_inj (a b: N)
+                      (E: NilZero.string_of_uint (N.to_uint a)
+                           =
+                          NilZero.string_of_uint (N.to_uint b)):
+  a = b.
+Proof.
+assert (UsuA := NilZero.usu (N.to_uint a) (to_uint_nonnil a)).
+assert (UsuB := NilZero.usu (N.to_uint b) (to_uint_nonnil b)).
+apply DecimalN.Unsigned.to_uint_inj.
+enough (Q: Some (N.to_uint a) = Some (N.to_uint b)) by now inversion Q.
+rewrite<- UsuA. rewrite<- UsuB.
+now rewrite E.
+Qed.
+
+Lemma make_var_name_inj (prefix: string) (a b: N)
+                        (E: make_var_name prefix a = make_var_name prefix b):
+  a = b.
+Proof.
+cbn in E. inversion E. apply string_of_N_inj.
+apply string_app_l_inj with (a := prefix). assumption.
+Qed.
+
+Lemma make_var_name_inj' (prefix: string) (a b: N)
+                         (NE: a <> b):
+  make_var_name prefix a <> make_var_name prefix b.
+Proof.
+intro E. apply NE.
+exact (make_var_name_inj prefix a b E).
+Qed.
