From40To50/Stmt.v
@@ -1,0 +1,2575 @@
+From Coq Require Import String NArith ZArith DecimalString List Lia Eqdep_dec.
+
+From Vyper Require Import Config Logic2 NaryFun.
+From Vyper.CheckArith Require Import Builtins.
+From Vyper.L10 Require Import Base.
+From Vyper.L40 Require AST.
+From Vyper.L50 Require AST.
+From Vyper.L50 Require Import Types Expr Stmt.
+
+From Vyper.L40Metered Require Import Interpret.
+
+From Vyper.From40To50 Require Import Translate Proto Mangle Expr.
+
+(* We always return exactly one value from every function.
+ *)
+Definition StmtResultsAgree {C: VyperConfig}
+                (r40: world_state * memory * option (stmt_result uint256))
+                (r50: world_state * string_map dynamic_value * option (stmt_result (list dynamic_value)))
+                (varcap: N)
+: Prop
+:= let '(w40, m40, v40) := r40 in
+   let '(w50, m50, v50) := r50 in
+   LocalVarsAgree m40 m50 varcap
+    /\
+   match v40, v50 with
+   | Some s40, Some s50 =>
+        match s40, s50 with
+        | StmtSuccess, StmtSuccess
+        | StmtAbort AbortBreak, StmtAbort AbortBreak
+        | StmtAbort AbortContinue, StmtAbort AbortContinue
+            => w40 = w50
+
+        | StmtAbort a40, StmtAbort a50 =>
+            get_world_except_memory w40 = get_world_except_memory w50
+             /\
+            a40 = a50
+        | StmtReturnFromFunction x40, StmtReturnFromFunction x50 =>
+               w40 = w50
+                /\
+               x50 = existT _ U256 (yul_uint256 x40) :: nil
+        | _, _ => False
+        end
+   | None, None => True
+   | _, _ => False
+   end.
+
+(** We have to demand that [mstore()] doesn't change anything except memory
+    otherwise the world changes in an unspecified way and everything is lost.
+ *)
+Definition BuiltinsSupportMstore {C: VyperConfig} (b: string -> option L50.Builtins.yul_builtin)
+:= match b "mstore"%string with
+   | None => False
+   | Some mstore =>
+      L50.Builtins.b_input_types mstore = U256 :: U256 :: nil
+       /\
+      L50.Builtins.b_output_types mstore = nil
+       /\
+      forall world addr value ArityOk,
+        match fst (nary_call (L50.Builtins.b_fun mstore world) (addr :: value :: nil) ArityOk) with
+        | (w, ExprSuccess nil) =>
+             mload w addr = value
+              /\
+             get_world_except_memory w = get_world_except_memory world
+        | _ => False (* mstore can't fail *)
+        end
+   end.
+
+(** [call_builtin] has a nasty dependent match inside for typechecking,
+    so this is less straightforward than it should be.
+ *)
+Lemma BuiltinsSupportMstore' {C: VyperConfig} (b: string -> option L50.Builtins.yul_builtin)
+                             (Ok: BuiltinsSupportMstore b):
+   match b "mstore"%string with
+   | None => False
+   | Some mstore =>
+      forall world addr value,
+          match L50.Builtins.call_builtin mstore world
+           (existT (fun t : yul_type => yul_value t) U256 (yul_uint256 addr)
+            :: existT (fun t : yul_type => yul_value t) U256 (yul_uint256 value) :: nil) 
+          with
+          | (w, ExprSuccess nil) =>
+               mload w addr = value
+                /\
+               get_world_except_memory w = get_world_except_memory world
+          | _ => False (* mstore can't fail *)
+          end
+   end.
+Proof.
+unfold BuiltinsSupportMstore in Ok.
+destruct (b "mstore"%string). 2:assumption.
+intros world addr value.
+unfold L50.Builtins.call_builtin.
+destruct Ok as (InputOk, (OutputOk, FunOk)).
+assert (TC: Builtins.mass_typecheck
+                (existT (fun t : yul_type => yul_value t) U256 (yul_uint256 addr)
+                 :: existT (fun t : yul_type => yul_value t) U256 (yul_uint256 value) :: nil)
+                (Builtins.b_input_types y)
+              = L50.Builtins.MassTypecheckOk)
+  by now rewrite InputOk.
+rewrite L50.Builtins.mass_typecheck_ok_rewrite with (Ok := TC). cbn.
+remember (Builtins.call_builtin_helper _ _ _) as foo. clear Heqfoo.
+assert (F := FunOk world addr value foo).
+destruct nary_call as ((w', e), rest).
+destruct e as [out | ab]; cbn in F. 2:contradiction.
+destruct out. 2:contradiction. now rewrite OutputOk.
+Qed.
+
+(** Here [revert()] is used to signal exceptions ([AbortException])
+    and to implement Fe's revert statement ([AbortRevert]).
+    The magical distinction between [revert(_, 0)] and [revert(_, 1)]
+    is unnatural from the EVM viewpoint but here we'll pretend that EVM
+    cares about Fe's raises and reverts.
+ *)
+Definition BuiltinsSupportRevert {C: VyperConfig} (b: string -> option L50.Builtins.yul_builtin)
+:= match b "revert"%string with
+   | None => False
+   | Some revert =>
+      L50.Builtins.b_input_types revert = U256 :: U256 :: nil
+       /\
+      L50.Builtins.b_output_types revert = nil
+       /\
+      (forall world addr ArityOk,
+        match fst (nary_call (L50.Builtins.b_fun revert world) (addr :: zero256 :: nil) ArityOk) with
+        | (w, ExprAbort AbortRevert) =>
+              w = world
+        | _ => False
+        end)
+       /\
+      forall world addr ArityOk,
+        match fst (nary_call (L50.Builtins.b_fun revert world) (addr :: one256 :: nil) ArityOk) with
+        | (w, ExprAbort (AbortException e)) =>
+              e = mload world addr /\ w = world
+        | _ => False
+        end
+   end.
+
+(* dup of BuiltinsSupportMstore' *)
+Lemma BuiltinsSupportRevert0 {C: VyperConfig} (b: string -> option L50.Builtins.yul_builtin)
+                             (Ok: BuiltinsSupportRevert b):
+   match b "revert"%string with
+   | None => False
+   | Some revert =>
+      forall world addr,
+          match L50.Builtins.call_builtin revert world
+           (existT (fun t : yul_type => yul_value t) U256 (yul_uint256 addr)
+            :: existT (fun t : yul_type => yul_value t) U256 (yul_uint256 zero256) :: nil) 
+          with
+          | (w, ExprAbort AbortRevert) => w = world
+          | _ => False
+          end
+   end.
+Proof.
+unfold BuiltinsSupportRevert in Ok.
+destruct (b "revert"%string). 2:assumption.
+intros world addr.
+unfold L50.Builtins.call_builtin.
+destruct Ok as (InputOk, (OutputOk, (FunOk, _))).
+assert (TC: Builtins.mass_typecheck
+                (existT (fun t : yul_type => yul_value t) U256 (yul_uint256 addr)
+                 :: existT (fun t : yul_type => yul_value t) U256 (yul_uint256 zero256) :: nil)
+                (Builtins.b_input_types y)
+              = L50.Builtins.MassTypecheckOk)
+  by now rewrite InputOk.
+rewrite L50.Builtins.mass_typecheck_ok_rewrite with (Ok := TC). cbn.
+remember (Builtins.call_builtin_helper _ _ _) as foo. clear Heqfoo.
+assert (F := FunOk world addr foo).
+destruct nary_call as ((w', e), rest).
+destruct e as [out | ab]; cbn in F. { contradiction. }
+now destruct ab.
+Qed.
+
+Lemma BuiltinsSupportRevert1 {C: VyperConfig} (b: string -> option L50.Builtins.yul_builtin)
+                             (Ok: BuiltinsSupportRevert b):
+   match b "revert"%string with
+   | None => False
+   | Some revert =>
+      forall world addr,
+          match L50.Builtins.call_builtin revert world
+           (existT (fun t : yul_type => yul_value t) U256 (yul_uint256 addr)
+            :: existT (fun t : yul_type => yul_value t) U256 (yul_uint256 one256) :: nil) 
+          with
+          | (w, ExprAbort (AbortException e)) => e = mload world addr /\ w = world
+          | _ => False 
+          end
+   end.
+Proof.
+unfold BuiltinsSupportRevert in Ok.
+destruct (b "revert"%string). 2:assumption.
+intros world addr.
+unfold L50.Builtins.call_builtin.
+destruct Ok as (InputOk, (OutputOk, (_, FunOk))).
+assert (TC: Builtins.mass_typecheck
+                (existT (fun t : yul_type => yul_value t) U256 (yul_uint256 addr)
+                 :: existT (fun t : yul_type => yul_value t) U256 (yul_uint256 zero256) :: nil)
+                (Builtins.b_input_types y)
+              = L50.Builtins.MassTypecheckOk)
+  by now rewrite InputOk.
+rewrite L50.Builtins.mass_typecheck_ok_rewrite with (Ok := TC). cbn.
+remember (Builtins.call_builtin_helper _ _ _) as foo. clear Heqfoo.
+assert (F := FunOk world addr foo).
+destruct nary_call as ((w', e), rest).
+destruct e as [out | ab]; cbn in F.  contradiction.
+now destruct ab.
+Qed.
+
+Definition BuiltinsSupportStop {C: VyperConfig} (b: string -> option L50.Builtins.yul_builtin)
+:= match b "stop"%string with
+   | None => False
+   | Some stop =>
+      L50.Builtins.b_input_types stop = nil
+       /\
+      L50.Builtins.b_output_types stop = nil
+       /\
+      forall world ArityOk,
+        match fst (nary_call (L50.Builtins.b_fun stop world) nil ArityOk) with
+        | (w, ExprAbort AbortReturnFromContract) => w = world
+        | _ => False
+        end
+   end.
+
+Lemma BuiltinsSupportStop' {C: VyperConfig} (b: string -> option L50.Builtins.yul_builtin)
+                           (Ok: BuiltinsSupportStop b):
+   match b "stop"%string with
+   | None => False
+   | Some stop =>
+      forall world,
+          match L50.Builtins.call_builtin stop world nil with
+          | (w, ExprAbort AbortReturnFromContract) => w = world
+          | _ => False
+          end
+   end.
+Proof.
+unfold BuiltinsSupportStop in Ok.
+destruct (b "stop"%string). 2:assumption.
+intros world.
+unfold L50.Builtins.call_builtin.
+destruct Ok as (InputOk, (OutputOk, FunOk)).
+assert (TC: Builtins.mass_typecheck nil (Builtins.b_input_types y)
+              = L50.Builtins.MassTypecheckOk)
+  by now rewrite InputOk.
+rewrite L50.Builtins.mass_typecheck_ok_rewrite with (Ok := TC). cbn.
+remember (Builtins.call_builtin_helper _ _ _) as foo. clear Heqfoo.
+assert (F := FunOk world foo).
+destruct nary_call as ((w', e), rest).
+destruct e as [out | ab]; cbn in F.  contradiction.
+now destruct ab.
+Qed.
+
+Definition BuiltinsSupportPop {C: VyperConfig} (b: string -> option L50.Builtins.yul_builtin)
+:= match b "pop"%string with
+   | None => False
+   | Some pop =>
+      L50.Builtins.b_input_types pop = U256 :: nil
+       /\
+      L50.Builtins.b_output_types pop = nil
+       /\
+      forall world value ArityOk,
+        match fst (nary_call (L50.Builtins.b_fun pop world) (value :: nil) ArityOk) with
+        | (w, ExprSuccess nil) => w = world
+        | _ => False
+        end
+   end.
+
+Lemma BuiltinsSupportPop' {C: VyperConfig} (b: string -> option L50.Builtins.yul_builtin)
+                          (Ok: BuiltinsSupportPop b):
+   match b "pop"%string with
+   | None => False
+   | Some pop =>
+      forall world value,
+          match L50.Builtins.call_builtin pop world
+                   (existT (fun t : yul_type => yul_value t) U256 (yul_uint256 value) :: nil) with
+          | (w, ExprSuccess nil) => w = world
+          | _ => False
+          end
+   end.
+Proof.
+unfold BuiltinsSupportPop in Ok.
+destruct (b "pop"%string). 2:assumption.
+intros world value.
+unfold L50.Builtins.call_builtin.
+destruct Ok as (InputOk, (OutputOk, FunOk)).
+assert (TC: Builtins.mass_typecheck 
+                (existT (fun t : yul_type => yul_value t) U256 (yul_uint256 value) :: nil) 
+                (Builtins.b_input_types y)
+              = L50.Builtins.MassTypecheckOk)
+  by now rewrite InputOk.
+rewrite L50.Builtins.mass_typecheck_ok_rewrite with (Ok := TC). cbn.
+remember (Builtins.call_builtin_helper _ _ _) as foo. clear Heqfoo.
+assert (F := FunOk world value foo).
+destruct nary_call as ((w', e), rest).
+destruct e as [out | ab]; cbn in F. 2:contradiction.
+destruct out. 2:contradiction.
+now rewrite OutputOk.
+Qed.
+
+Definition BuiltinsSupportBasics {C: VyperConfig} (b: string -> option L50.Builtins.yul_builtin)
+:= BuiltinsSupportMstore b
+    /\
+   BuiltinsSupportRevert b
+    /\
+   BuiltinsSupportStop b
+    /\
+   BuiltinsSupportPop b.
+
+Record SecondaryVarsOk {C: VyperConfig} (loop_info: list L40.Expr.loop_ctx)
+                       (loc: string_map dynamic_value)
+:= { sv_result_declared:
+           (* The local var dictionary contains [$$result] of type [u256].
+            All translated functions declare [$$result] as the output variable
+            and interpret_call binds all outputs to zeros. 
+           *)
+           match map_lookup loc "$$result" with
+           | Some (existT _ (IntType I256 false (* that's U256 *) ) _) => True
+           | _ => False
+           end;
+     sv_offsets_agree: LoopOffsetsAgree loop_info loc;
+     sv_cursors_agree: LoopCursorsAgree loop_info loc;
+     sv_offsets_undeclared: forall k, List.length loop_info <= k ->
+                              map_lookup loc (make_var_name "offset" (N.of_nat k)) = None;
+     sv_cursors_undeclared: forall k, List.length loop_info <= k ->
+                              map_lookup loc (make_var_name "cursor" (N.of_nat k)) = None;
+   }.
+Arguments sv_result_declared {_ _ _}.
+Arguments sv_offsets_agree {_ _ _}.
+Arguments sv_cursors_agree {_ _ _}.
+Arguments sv_offsets_undeclared {_ _ _}.
+Arguments sv_cursors_undeclared {_ _ _}.
+
+Lemma interpret_translated_small_stmt {C: VyperConfig}
+                                      {B: builtin_names_config}
+                                      {protos: string_map proto}
+                                      {ss40: L40.AST.small_stmt}
+                                      {s50: list L50.AST.stmt}
+                                      {loop_depth: N}
+                                      {max_loop_iterations: nat}
+                                      (call40: forall
+                                                    (decl: L40.AST.decl)
+                                                    (world: world_state)
+                                                    (arg_values: list uint256),
+                                                  world_state * option (expr_result uint256))
+                                      (call50: forall
+                                                    (decl: L50.AST.fun_decl)
+                                                    (world: world_state)
+                                                    (arg_values: list dynamic_value),
+                                                  world_state * option (expr_result (list dynamic_value)))
+                                      (CallsOk: forall (decl40: L40.AST.decl)
+                                                       (decl50: L50.AST.fun_decl)
+                                                       (Ok: translate_fun_decl B protos decl40 = inr decl50)
+                                                       (world: world_state)
+                                                       (args40: list uint256)
+                                                       (args50: list dynamic_value)
+                                                       (ArgsOk: args50 = map (fun x : uint256 => existT (fun t : yul_type => yul_value t) U256 (yul_uint256 x)) args40),
+                                                   ResultsAgree (call40 decl40 world args40)
+                                                                (call50 decl50 world args50) 1%N)
+                                      (decls40: string_map L40.AST.decl)
+                                      (decls50: string_map L50.AST.fun_decl)
+                                      (this_fun_decl40: option L40.AST.decl)
+                                      (this_fun_decl50: option L50.AST.fun_decl)
+                                      (FunDeclOk: match this_fun_decl40, this_fun_decl50 with
+                                                  | Some d40, Some d50 =>
+                                                      translate_fun_decl B protos d40 = inr d50
+                                                  | None, None => True
+                                                  | _, _ => False
+                                                  end)
+                                      (Ok: translate_small_stmt (match this_fun_decl50 with
+                                                                 | Some _ => true
+                                                                 | None => false
+                                                                 end) protos ss40 loop_depth = inr s50)
+                                      (DeclsOk: translate_fun_decls B protos decls40 = inr decls50)
+                                      (builtins40: string -> option builtin)
+                                      (builtins50: string -> option L50.Builtins.yul_builtin)
+                                      (BuiltinsOk: AllBuiltinsAgreeIfU256 builtins40 builtins50)
+                                      (BuiltinsBasics: BuiltinsSupportBasics builtins50)
+                                      (BuiltinsSafe: forall x,
+                                                       builtins50 ("$" ++ x)%string = None)
+                                      (ProtosOk: ProtosAgree (map_lookup protos) builtins50)
+                                      (world: world_state)
+                                      (loc40: memory)
+                                      (loc50: string_map dynamic_value)
+                                      (varcap: N)
+                                      (VarcapOk: (L40.AST.var_cap_small_stmt ss40 <= varcap)%N)
+                                      (LocalVarsOk: LocalVarsAgree loc40 loc50 varcap)
+                                      (loop_info: list L40.Expr.loop_ctx)
+                                      (LoopDepthOk: length loop_info = N.to_nat loop_depth)
+                                      (SV: SecondaryVarsOk loop_info loc50):
+  let '(w, l, result50) :=
+    interpret_stmt_list max_loop_iterations builtins50 (map_lookup decls50) 
+                        this_fun_decl50 call50 world loc50 s50
+  in
+    StmtResultsAgree
+      (interpret_small_stmt_metered decls40 call40 builtins40 world loc40 loop_info ss40)
+      (w, l, result50)
+      varcap
+     /\
+    SecondaryVarsOk loop_info l.
+Proof.
+destruct BuiltinsBasics as (SupportMstore, (SupportRevert, (SupportStop, SupportPop))).
+destruct ss40; cbn.
+{ (* abort *)
+  destruct ab; inversion Ok; subst s50; clear Ok; cbn.
+  { (* exception *)
+    (* do mstore *)
+    assert (SupportMstore' := BuiltinsSupportMstore' builtins50 SupportMstore).
+    destruct (builtins50 "mstore"%string) as [mstore|]. 2:contradiction.
+    rewrite (unmangled_names_are_not_translated decls40 decls50 DeclsOk "mstore" eq_refl).
+    assert (SupportMstore'' := SupportMstore' world zero256 data).
+    destruct L50.Builtins.call_builtin as (w, [out | ab]). 2:contradiction.
+    destruct out. 2:contradiction.
+    (* do revert *)
+    assert (SupportRevert' := BuiltinsSupportRevert1 builtins50 SupportRevert).
+    destruct (builtins50 "revert"%string) as [revert|]. 2:contradiction.
+    rewrite (unmangled_names_are_not_translated decls40 decls50 DeclsOk "revert" eq_refl).
+    assert (SupportRevert'' := SupportRevert' w zero256).
+    destruct L50.Builtins.call_builtin as (w', [out | ab]). { contradiction. }
+    destruct ab; try contradiction.
+    destruct SupportRevert'' as (RevertDataOk, RevertWorldOk).
+    destruct SupportMstore'' as (MstoreDataOk, MstoreWorldOk).
+    symmetry in MstoreWorldOk.
+    now subst.
+  }
+  { (* break *) easy. }
+  { (* continue *) easy. }
+  { (* return from contract *)
+    assert (SupportStop' := BuiltinsSupportStop' builtins50 SupportStop).
+    destruct (builtins50 "stop"%string) as [stop|]. 2:contradiction.
+    rewrite (unmangled_names_are_not_translated decls40 decls50 DeclsOk "stop" eq_refl).
+    assert (SupportStop'' := SupportStop' world).
+    destruct L50.Builtins.call_builtin as (w', [out | ab]). { contradiction. }
+    destruct ab; try contradiction. now subst.
+  }
+  { (* revert *)
+    assert (SupportRevert' := BuiltinsSupportRevert0 builtins50 SupportRevert).
+    destruct (builtins50 "revert"%string) as [revert|]. 2:contradiction.
+    rewrite (unmangled_names_are_not_translated decls40 decls50 DeclsOk "revert" eq_refl).
+    assert (SupportRevert'' := SupportRevert' world zero256).
+    destruct L50.Builtins.call_builtin as (w', [out | ab]). { contradiction. }
+    destruct ab; try contradiction. now subst.
+  }
+}
+{ (* return from function *)
+  destruct this_fun_decl50 as [this_fd|]. 2:easy. (* returns only allowed within functions *)
+  cbn in Ok.
+  remember (translate_expr protos e loop_depth) as e'.
+  destruct e' as [|(e', n')]. { easy. }
+  destruct n' as [|p].
+  {
+    (* return with a builtin that produces 0 values - legal in Fe *)
+    inversion Ok; subst s50; clear Ok; cbn.
+    symmetry in Heqe'.
+    assert (ReturnValueOk := interpret_translated_expr Heqe' call40 call50 CallsOk decls40 decls50 DeclsOk
+                                                             builtins40 builtins50 BuiltinsOk BuiltinsSafe
+                                                             ProtosOk world loc40 loc50
+                                                             (local_vars_agree_weaken VarcapOk LocalVarsOk)
+                                                             loop_info LoopDepthOk
+                                                             (sv_offsets_agree SV) (sv_cursors_agree SV)).
+    unfold ResultsAgree in ReturnValueOk.
+    destruct (interpret_expr_metered decls40 call40 builtins40 world loc40 loop_info e) as (w40, r40).
+    destruct (interpret_expr builtins50 (map_lookup decls50) call50 world loc50 e') as (w50, r50).
+    destruct r40 as [r40|], r50 as [r50|]; try easy. (* dealing with None (out of limits) *)
+    unfold ExprResultsAgree in ReturnValueOk.
+    destruct ReturnValueOk as (W, ReturnValueOk). subst w40.
+    destruct r40 as [v40|ab40], r50 as [v50|ab50]; try easy.
+    destruct v50. 2:{
+      destruct v50. 2:tauto. assert (Bad: 0%N = 1%N) by tauto. discriminate.
+    }
+
+    (* pass the check that $$result is declared at all *)
+    assert (ResultDeclared := sv_result_declared SV).
+    destruct (map_lookup loc50 "$$result") as [(result_type, _)|]. 2:contradiction.
+    destruct result_type; try contradiction.
+    destruct size; try contradiction.
+    destruct signed; try contradiction.
+    destruct yul_type_eq_dec; try easy.
+
+    (* fetch the declaration of $$result *)
+    destruct this_fun_decl40 as [this_fd40|]. 2:contradiction.
+    unfold translate_fun_decl in FunDeclOk.
+    destruct this_fd40 as (this_fun_name, this_fun_arity, this_fun_body40).
+    remember (translate_block true B protos this_fun_body40 0) as this_fun_body50.
+    destruct this_fun_body50 as [|(this_fun_body50)]. 1:discriminate.
+    inversion FunDeclOk; subst this_fd; clear FunDeclOk. cbn.
+
+    (* finally we can load $$result. *)
+    unfold map_lookup. unfold map_insert. rewrite Map.insert_ok.
+    destruct string_dec. 2:contradiction. cbn.
+    destruct ReturnValueOk as (V, _).
+    split.
+    {
+      split. 2:now subst.
+      cbn in LocalVarsOk.
+
+      (* we need to prove that setting $$result doesn't disturb LocalVarsAgree. *)
+      unfold LocalVarsAgree in *.
+      intros k L. assert (A := LocalVarsOk k L).
+      unfold map_lookup in *. rewrite Map.insert_ok.
+      destruct (string_dec "$$result" (make_var_name "var" k)) as [E|NE]. 2:assumption.
+      exfalso. cbn in E. discriminate.
+    }
+    split.
+    {
+      unfold map_lookup. rewrite Map.insert_ok.
+      now destruct string_dec.
+    }
+    {
+      unfold LoopOffsetsAgree. intros k L.
+      unfold map_lookup. rewrite Map.insert_ok.
+      destruct (string_dec "$$result" (make_var_name "offset" (N.of_nat k))) as [E|NE].
+      2:exact (sv_offsets_agree SV k L).
+      exfalso. cbn in E. discriminate.
+    }
+    {
+      unfold LoopCursorsAgree. intros k L.
+      unfold map_lookup. rewrite Map.insert_ok.
+      destruct (string_dec "$$result" (make_var_name "cursor" (N.of_nat k))) as [E|NE].
+      2:exact (sv_cursors_agree SV k L).
+      exfalso. cbn in E. discriminate.
+    }
+    {
+      intros k GE. unfold map_lookup.
+      rewrite Map.insert_ok.
+      destruct (string_dec "$$result" (make_var_name "offset" (N.of_nat k))) as [E|NE].
+      2:exact (sv_offsets_undeclared SV k GE).
+      exfalso. cbn in E. discriminate.
+    }
+    intros k GE. unfold map_lookup.
+    rewrite Map.insert_ok.
+    destruct (string_dec "$$result" (make_var_name "cursor" (N.of_nat k))) as [E|NE].
+    2:exact (sv_cursors_undeclared SV k GE).
+    exfalso. cbn in E. discriminate.
+    subst ab50. now destruct ab40.
+  }
+  (* normal return with something that produces a value *)
+  (* dup *)
+  destruct p; try discriminate.
+  inversion Ok; subst s50; clear Ok; cbn.
+  symmetry in Heqe'.
+  assert (ReturnValueOk := interpret_translated_expr Heqe' call40 call50 CallsOk decls40 decls50 DeclsOk
+                                                           builtins40 builtins50 BuiltinsOk BuiltinsSafe
+                                                           ProtosOk world loc40 loc50
+                                                           (local_vars_agree_weaken VarcapOk LocalVarsOk)
+                                                           loop_info LoopDepthOk
+                                                           (sv_offsets_agree SV) (sv_cursors_agree SV)).
+  unfold ResultsAgree in ReturnValueOk.
+  destruct (interpret_expr_metered decls40 call40 builtins40 world loc40 loop_info e) as (w40, r40).
+  destruct (interpret_expr builtins50 (map_lookup decls50) call50 world loc50 e') as (w50, r50).
+  destruct r40 as [r40|], r50 as [r50|]; try easy. (* dealing with None (out of limits) *)
+  unfold ExprResultsAgree in ReturnValueOk.
+  destruct ReturnValueOk as (W, ReturnValueOk). subst w40.
+  destruct r40 as [v40|ab40], r50 as [v50|ab50]; try easy.
+  destruct v50 as [|v]. { destruct ReturnValueOk as (_, A). discriminate. }
+  destruct v50. 2:tauto.
+
+  (* pass the check that $$result is declared at all *)
+  assert (ResultDeclared := sv_result_declared SV).
+  destruct (map_lookup loc50 "$$result") as [(result_type, _)|]. 2:contradiction.
+  destruct result_type; try contradiction.
+  destruct size; try contradiction.
+  destruct signed; try contradiction.
+  destruct ReturnValueOk as (V, _). subst v.
+  destruct yul_type_eq_dec; try easy.
+
+  (* fetch the declaration of $$result *)
+  destruct this_fun_decl40 as [this_fd40|]. 2:contradiction.
+  unfold translate_fun_decl in FunDeclOk.
+  destruct this_fd40 as (this_fun_name, this_fun_arity, this_fun_body40).
+  remember (translate_block true B protos this_fun_body40 0) as this_fun_body50.
+  destruct this_fun_body50 as [|(this_fun_body50)]. 1:discriminate.
+  inversion FunDeclOk; subst this_fd; clear FunDeclOk. cbn.
+
+  (* finally we can load $$result. *)
+  unfold map_lookup. unfold map_insert. rewrite Map.insert_ok.
+  destruct string_dec. 2:contradiction. cbn.
+  split.
+  {
+    split. 2:now subst.
+    cbn in LocalVarsOk.
+
+    (* we need to prove that setting $$result doesn't disturb LocalVarsAgree. *)
+    unfold LocalVarsAgree in *.
+    intros k L. assert (A := LocalVarsOk k L).
+    unfold map_lookup in *. rewrite Map.insert_ok.
+    destruct (string_dec "$$result" (make_var_name "var" k)) as [E|NE]. 2:assumption.
+    exfalso. cbn in E. discriminate.
+  }
+  split.
+  {
+    unfold map_lookup. rewrite Map.insert_ok.
+    now destruct string_dec.
+  }
+  {
+    unfold LoopOffsetsAgree. intros k L.
+    unfold map_lookup. rewrite Map.insert_ok.
+    destruct (string_dec "$$result" (make_var_name "offset" (N.of_nat k))) as [E|NE].
+    2:exact (sv_offsets_agree SV k L).
+    exfalso. cbn in E. discriminate.
+  }
+  {
+    unfold LoopCursorsAgree. intros k L.
+    unfold map_lookup. rewrite Map.insert_ok.
+    destruct (string_dec "$$result" (make_var_name "cursor" (N.of_nat k))) as [E|NE].
+    2:exact (sv_cursors_agree SV k L).
+    exfalso. cbn in E. discriminate.
+  }
+  {
+    intros k GE. unfold map_lookup.
+    rewrite Map.insert_ok.
+    destruct (string_dec "$$result" (make_var_name "offset" (N.of_nat k))) as [E|NE].
+    2:exact (sv_offsets_undeclared SV k GE).
+    exfalso. cbn in E. discriminate.
+  }
+  intros k GE. unfold map_lookup.
+  rewrite Map.insert_ok.
+  destruct (string_dec "$$result" (make_var_name "cursor" (N.of_nat k))) as [E|NE].
+  2:exact (sv_cursors_undeclared SV k GE).
+  exfalso. cbn in E. discriminate.
+  subst ab50. now destruct ab40.
+}
+{ (* raise *)
+  cbn in Ok. remember (translate_expr protos e loop_depth) as e'.
+  destruct e' as [err|(e50, n')]. 1:discriminate. symmetry in Heqe'.
+  destruct n' as [|p].
+  { (* 0 results *)
+    inversion Ok; subst s50; clear Ok. cbn.
+
+    (* ensure that both sides evaluate to 0 *)
+    assert (RaisedValueOk := interpret_translated_expr Heqe' call40 call50 CallsOk decls40 decls50 DeclsOk
+                                                             builtins40 builtins50 BuiltinsOk BuiltinsSafe
+                                                             ProtosOk world loc40 loc50
+                                                             (local_vars_agree_weaken VarcapOk LocalVarsOk)
+                                                             loop_info LoopDepthOk
+                                                             (sv_offsets_agree SV) (sv_cursors_agree SV)).
+    unfold ResultsAgree in RaisedValueOk.
+    destruct (interpret_expr_metered decls40 call40 builtins40 world loc40 loop_info e) as (w40, r40).
+    destruct (interpret_expr builtins50 (map_lookup decls50) call50 world loc50 e50) as (w50, r50).
+    destruct r40 as [r40|], r50 as [r50|]; try easy.
+    destruct RaisedValueOk as (W, RaisedValuesAgree). subst w40.
+    unfold ExprResultsAgree in RaisedValuesAgree.
+    destruct r40 as [val40 | ab40], r50 as [val50 | ab50]; try contradiction.
+    2:{ subst ab50. subst. now destruct ab40. }
+    destruct val50.
+    2:{ destruct val50. { assert (Bad: 0%N = 1%N) by tauto. discriminate. } contradiction. }
+    destruct RaisedValuesAgree as (V, _). subst val40.
+
+    (* dup from abort above - doing mstore *)
+    assert (SupportMstore' := BuiltinsSupportMstore' builtins50 SupportMstore).
+    destruct (builtins50 "mstore"%string) as [mstore|]. 2:contradiction.
+    rewrite (unmangled_names_are_not_translated decls40 decls50 DeclsOk "mstore" eq_refl).
+    assert (SupportMstore'' := SupportMstore' w50 zero256 zero256).
+    destruct L50.Builtins.call_builtin as (w, [out | ab]). 2:contradiction.
+    destruct out. 2:contradiction.
+    (* do revert *)
+    assert (SupportRevert' := BuiltinsSupportRevert1 builtins50 SupportRevert).
+    destruct (builtins50 "revert"%string) as [revert|]. 2:contradiction.
+    rewrite (unmangled_names_are_not_translated decls40 decls50 DeclsOk "revert" eq_refl).
+    assert (SupportRevert'' := SupportRevert' w zero256).
+    destruct L50.Builtins.call_builtin as (w', [out | ab]). { contradiction. }
+    destruct ab; try contradiction.
+    destruct SupportMstore'' as (MstoreDataOk, MstoreWorldOk).
+    destruct SupportRevert'' as (RevertDataOk, RevertWorldOk).
+    rewrite MstoreDataOk in RevertDataOk. subst.
+    now unfold StmtResultsAgree.
+  }
+  (* raising 1 value; massive dup of course. *)
+  destruct p; try discriminate.
+  inversion Ok; subst s50; clear Ok; cbn.
+  assert (RaisedValueOk := interpret_translated_expr Heqe' call40 call50 CallsOk decls40 decls50 DeclsOk
+                                                             builtins40 builtins50 BuiltinsOk BuiltinsSafe
+                                                             ProtosOk world loc40 loc50
+                                                             (local_vars_agree_weaken VarcapOk LocalVarsOk)
+                                                             loop_info LoopDepthOk
+                                                             (sv_offsets_agree SV) (sv_cursors_agree SV)).
+  unfold ResultsAgree in RaisedValueOk.
+  destruct (interpret_expr_metered decls40 call40 builtins40 world loc40 loop_info e) as (w40, r40).
+  destruct (interpret_expr builtins50 (map_lookup decls50) call50 world loc50 e50) as (w50, r50).
+  destruct r40 as [r40|], r50 as [r50|]; try easy.
+  2:{
+    (* both computations resulted in out of limits error *)
+    (* we still have to check for mstore *)
+    assert (SupportMstore' := BuiltinsSupportMstore' builtins50 SupportMstore).
+    destruct (builtins50 "mstore"%string) as [mstore|]. 2:contradiction.
+    cbn. rewrite (unmangled_names_are_not_translated decls40 decls50 DeclsOk "mstore" eq_refl).
+    tauto.
+  }
+  unfold StmtResultsAgree.
+  destruct RaisedValueOk as (W, RaisedValuesAgree). subst w40.
+  unfold ExprResultsAgree in RaisedValuesAgree.
+
+  (* doing mstore - 1*)
+  assert (SupportMstore' := BuiltinsSupportMstore' builtins50 SupportMstore).
+  destruct (builtins50 "mstore"%string) as [mstore|]. 2:contradiction.
+  rewrite (unmangled_names_are_not_translated decls40 decls50 DeclsOk "mstore" eq_refl).
+
+  destruct r40 as [val40 | ab40], r50 as [val50 | ab50]; try easy.
+  2:{ subst ab50. now destruct ab40. }
+  cbn.
+  destruct val50.
+  { assert (Bad: 1%N = 0%N) by tauto. discriminate. }
+  destruct val50. 2: contradiction.
+  destruct RaisedValuesAgree as (V, _). subst.
+
+  (* doing mstore - 2 *)
+  assert (SupportMstore'' := SupportMstore' w50 zero256 val40).
+  destruct L50.Builtins.call_builtin as (w, [out | ab]). 2:contradiction.
+  destruct out. 2:contradiction.
+
+  (* do revert *)
+  assert (SupportRevert' := BuiltinsSupportRevert1 builtins50 SupportRevert).
+  destruct (builtins50 "revert"%string) as [revert|]. 2:contradiction.
+  rewrite (unmangled_names_are_not_translated decls40 decls50 DeclsOk "revert" eq_refl).
+  assert (SupportRevert'' := SupportRevert' w zero256).
+  destruct L50.Builtins.call_builtin as (w', [out | ab]). { contradiction. }
+  destruct ab; try contradiction.
+  destruct SupportMstore'' as (MstoreDataOk, MstoreWorldOk).
+  destruct SupportRevert'' as (RevertDataOk, RevertWorldOk).
+  rewrite MstoreDataOk in RevertDataOk. subst.
+  now unfold StmtResultsAgree.
+}
+{ (* assign *)
+  cbn in Ok. remember (translate_expr protos rhs loop_depth) as rhs'.
+  destruct rhs' as [err|(rhs50, n')]. 1:discriminate. symmetry in Heqrhs'.
+  destruct n' as [|p].
+  { (* 0 results *)
+    cbn in Ok. inversion Ok; subst s50; clear Ok. cbn. cbn in LocalVarsOk. cbn in VarcapOk.
+    assert (AssignedValueOk := interpret_translated_expr Heqrhs' call40 call50 CallsOk decls40 decls50 DeclsOk
+                                                         builtins40 builtins50 BuiltinsOk BuiltinsSafe
+                                                         ProtosOk world loc40 loc50
+                                                         (local_vars_agree_weaken_right
+                                                           (local_vars_agree_weaken VarcapOk LocalVarsOk))
+                                                         loop_info LoopDepthOk
+                                                         (sv_offsets_agree SV) (sv_cursors_agree SV)).
+    unfold ResultsAgree in AssignedValueOk.
+    destruct (interpret_expr_metered decls40 call40 builtins40 world loc40 loop_info rhs) as (w40, r40).
+    destruct (interpret_expr builtins50 (map_lookup decls50) call50 world loc50 rhs50) as (w50, r50).
+    destruct AssignedValueOk as (W, AssignedValueOk). subst w40.
+    destruct r40 as [r40 | ], r50 as [r50 | ]; try easy.
+    unfold ExprResultsAgree in AssignedValueOk.
+
+    destruct r40 as [val40 | ab40], r50 as [val50 | ab50]; try easy. 
+    2:{ subst ab50. now destruct ab40. }
+    cbn.
+    destruct val50.
+    2:{ destruct val50. { assert (Bad: 0%N = 1%N) by tauto. discriminate. } contradiction. }
+    destruct AssignedValueOk as (V, _). subst.
+    assert (LhsOk := local_vars_agree_weaken_left (local_vars_agree_weaken VarcapOk LocalVarsOk) lhs (N.lt_succ_diag_r _)).
+    unfold LocalVarsAgree in LhsOk.
+    cbn in LhsOk. rewrite LhsOk.
+    destruct (yul_type_eq_dec U256 U256) as [E|]. 2:contradiction. clear E.
+    cbn.
+
+    split.
+    {
+      split. 2:trivial.
+      (* goal: LocalVarsAgree between OpenArray.put and Map.insert *)
+      intros k L.
+      unfold map_lookup. unfold map_insert. rewrite Map.insert_ok. rewrite OpenArray.put_ok.
+      remember (lhs =? k)%N as q. symmetry in Heqq. destruct q.
+      { (* lhs = k *)
+        apply N.eqb_eq in Heqq. subst lhs.
+        destruct string_dec as [_|NE]; trivial. cbn in NE. tauto.
+      }
+      (* lhs <> k *)
+      destruct string_dec as [E|_]; trivial.
+      {
+        rewrite N.eqb_neq in Heqq.
+        assert (M := make_var_name_inj' "var" lhs k Heqq).
+        easy.
+      }
+      apply (LocalVarsOk k L).
+    }
+    split.
+    {
+      unfold map_lookup. unfold map_insert. rewrite Map.insert_ok.
+      destruct string_dec as [E|NE]. { discriminate. }
+      apply (sv_result_declared SV).
+    }
+    {
+      unfold LoopOffsetsAgree. intros k L.
+      unfold map_lookup. unfold map_insert. rewrite Map.insert_ok.
+      destruct string_dec as [E|NE].
+      2:exact (sv_offsets_agree SV k L).
+      exfalso. cbn in E. discriminate.
+    } 
+    {
+      unfold LoopOffsetsAgree. intros k L.
+      unfold map_lookup. unfold map_insert. rewrite Map.insert_ok.
+      destruct string_dec as [E|NE].
+      2:exact (sv_cursors_agree SV k L).
+      exfalso. cbn in E. discriminate.
+    }
+    {
+      intros k GE. unfold map_lookup. unfold map_insert.
+      rewrite Map.insert_ok.
+      destruct string_dec as [E|NE].
+      2:exact (sv_offsets_undeclared SV k GE).
+      exfalso. cbn in E. discriminate.
+    }
+    intros k GE. unfold map_lookup. unfold map_insert.
+    rewrite Map.insert_ok.
+    destruct string_dec as [E|NE].
+    2:exact (sv_cursors_undeclared SV k GE).
+    exfalso. cbn in E. discriminate.
+  }
+  destruct p; try discriminate.
+  (* 1 result, of course dup from 0 results *)
+  cbn in Ok. inversion Ok; subst s50; clear Ok. cbn. cbn in LocalVarsOk. cbn in VarcapOk.
+  assert (AssignedValueOk := interpret_translated_expr Heqrhs' call40 call50 CallsOk decls40 decls50 DeclsOk
+                                                       builtins40 builtins50 BuiltinsOk BuiltinsSafe
+                                                       ProtosOk world loc40 loc50 
+                                                       (local_vars_agree_weaken_right
+                                                         (local_vars_agree_weaken VarcapOk LocalVarsOk))
+                                                       loop_info LoopDepthOk
+                                                       (sv_offsets_agree SV) (sv_cursors_agree SV)).
+  unfold ResultsAgree in AssignedValueOk.
+  destruct (interpret_expr_metered decls40 call40 builtins40 world loc40 loop_info rhs) as (w40, r40).
+  destruct (interpret_expr builtins50 (map_lookup decls50) call50 world loc50 rhs50) as (w50, r50).
+  destruct AssignedValueOk as (W, AssignedValueOk). subst w40.
+  unfold StmtResultsAgree.
+  destruct r40 as [r40 | ], r50 as [r50 | ]; try easy.
+  unfold ExprResultsAgree in AssignedValueOk.
+
+  destruct r40 as [val40 | ab40], r50 as [val50 | ab50]; try easy. 
+  2:{ subst ab50. now destruct ab40. }
+  cbn.
+  destruct val50. { assert (Bad: 1%N = 0%N) by tauto. discriminate. }
+  destruct val50. 2:contradiction.
+  destruct AssignedValueOk as (V, _). subst.
+  assert (LhsOk := local_vars_agree_weaken_left (local_vars_agree_weaken VarcapOk LocalVarsOk) lhs (N.lt_succ_diag_r _)).
+  unfold LocalVarsAgree in LhsOk.
+  cbn in LhsOk. 
+  cbn.
+  rewrite LhsOk.
+  destruct (yul_type_eq_dec U256 U256) as [E|]. 2:contradiction. clear E.
+  cbn.
+
+  split.
+  {
+    split. 2:trivial.
+    (* goal: LocalVarsAgree between OpenArray.put and Map.insert *)
+    intros k L.
+    unfold map_lookup. unfold map_insert. rewrite Map.insert_ok. rewrite OpenArray.put_ok.
+    remember (lhs =? k)%N as q. symmetry in Heqq. destruct q.
+    { (* lhs = k *)
+      apply N.eqb_eq in Heqq. subst lhs.
+      destruct string_dec as [_|NE]; trivial. cbn in NE. tauto.
+    }
+    (* lhs <> k *)
+    destruct string_dec as [E|_]; trivial.
+    {
+      rewrite N.eqb_neq in Heqq.
+      assert (M := make_var_name_inj' "var" lhs k Heqq).
+      easy.
+    }
+    apply (LocalVarsOk k L).
+  }
+  split.
+  {
+    unfold map_lookup. unfold map_insert. rewrite Map.insert_ok.
+    destruct string_dec as [E|NE]. { discriminate. }
+    apply (sv_result_declared SV).
+  }
+  {
+    unfold LoopOffsetsAgree. intros k L.
+    unfold map_lookup. unfold map_insert. rewrite Map.insert_ok.
+    destruct string_dec as [E|NE].
+    2:exact (sv_offsets_agree SV k L).
+    exfalso. cbn in E. discriminate.
+  } 
+  {
+    unfold LoopOffsetsAgree. intros k L.
+    unfold map_lookup. unfold map_insert. rewrite Map.insert_ok.
+    destruct string_dec as [E|NE].
+    2:exact (sv_cursors_agree SV k L).
+    exfalso. cbn in E. discriminate.
+  }
+  {
+    intros k GE. unfold map_lookup. unfold map_insert.
+    rewrite Map.insert_ok.
+    destruct string_dec as [E|NE].
+    2:exact (sv_offsets_undeclared SV k GE).
+    exfalso. cbn in E. discriminate.
+  }
+  intros k GE. unfold map_lookup. unfold map_insert.
+  rewrite Map.insert_ok.
+  destruct string_dec as [E|NE].
+  2:exact (sv_cursors_undeclared SV k GE).
+  exfalso. cbn in E. discriminate.
+}
+(* expr *)
+cbn in Ok. remember (translate_expr protos e loop_depth) as e'.
+destruct e' as [err|(e50, n')]. 1:discriminate. symmetry in Heqe'.
+destruct n' as [|p].
+{ (* 0 results *)
+  cbn in Ok. inversion Ok; subst s50; clear Ok. cbn. cbn in LocalVarsOk.
+  assert (ValueOk := interpret_translated_expr Heqe' call40 call50 CallsOk decls40 decls50 DeclsOk
+                                               builtins40 builtins50 BuiltinsOk BuiltinsSafe
+                                               ProtosOk world loc40 loc50
+                                               (local_vars_agree_weaken VarcapOk LocalVarsOk)
+                                               loop_info LoopDepthOk
+                                               (sv_offsets_agree SV) (sv_cursors_agree SV)).
+  unfold ResultsAgree in ValueOk.
+  destruct (interpret_expr_metered decls40 call40 builtins40 world loc40 loop_info e) as (w40, r40).
+  destruct (interpret_expr builtins50 (map_lookup decls50) call50 world loc50 e50) as (w50, r50).
+  destruct ValueOk as (W, ValueOk). subst w40.
+  unfold StmtResultsAgree.
+
+  destruct r40 as [r40 | ], r50 as [r50 | ]; try easy.
+  unfold ExprResultsAgree in ValueOk.
+  destruct r40 as [val40 | ab40], r50 as [val50 | ab50]; try easy.
+  2:{ subst ab50. now destruct ab40. }
+  cbn.
+  destruct val50.
+  2:{ destruct val50. { assert (Bad: 0%N = 1%N) by tauto. discriminate. } contradiction. }
+  destruct ValueOk as (V, _). subst.
+  cbn. now split.
+}
+destruct p; try discriminate.
+(* 1 result *)
+cbn in Ok. inversion Ok; subst s50; clear Ok. cbn. cbn in LocalVarsOk.
+assert (ValueOk := interpret_translated_expr Heqe' call40 call50 CallsOk decls40 decls50 DeclsOk
+                                             builtins40 builtins50 BuiltinsOk BuiltinsSafe
+                                             ProtosOk world loc40 loc50
+                                             (local_vars_agree_weaken VarcapOk LocalVarsOk)
+                                             loop_info LoopDepthOk
+                                             (sv_offsets_agree SV) (sv_cursors_agree SV)).
+unfold ResultsAgree in ValueOk.
+destruct (interpret_expr_metered decls40 call40 builtins40 world loc40 loop_info e) as (w40, r40).
+destruct (interpret_expr builtins50 (map_lookup decls50) call50 world loc50 e50) as (w50, r50).
+destruct ValueOk as (W, ValueOk). subst w40.
+
+(* do pop *)
+assert (SupportPop' := BuiltinsSupportPop' builtins50 SupportPop).
+destruct (builtins50 "pop"%string) as [pop|]. 2:contradiction.
+rewrite (unmangled_names_are_not_translated decls40 decls50 DeclsOk "pop" eq_refl).
+
+unfold StmtResultsAgree.
+unfold ExprResultsAgree in ValueOk.
+destruct r40 as [r40 | ], r50 as [r50 | ]; try easy.
+cbn.
+destruct r40 as [val40 | ab40], r50 as [val50 | ab50]; try easy.
+2:{ subst ab50. now destruct ab40. }
+cbn.
+destruct val50. { assert (Bad: 1%N = 0%N) by tauto. discriminate. }
+destruct val50. 2:contradiction.
+destruct ValueOk as (V, _). subst.
+assert (SupportPop'' := SupportPop' w50 val40).
+destruct (Builtins.call_builtin pop) as (w, [out | ab]). 2:contradiction.
+destruct out. 2:contradiction.
+subst w50. cbn.
+now split.
+Qed.
+
+Lemma lookup_unbind {C: VyperConfig}
+                    (loc50: string_map dynamic_value)
+                    (vars: list L50.AST.typename)
+                    (name: string):
+  map_lookup (LocalVars.unbind_vars vars loc50) name
+   =
+  if ListSet.set_mem string_dec name (List.map snd vars)
+    then None
+    else map_lookup loc50 name.
+Proof.
+revert loc50. induction vars as [|head]; intros. { easy. }
+unfold map_lookup in *. cbn.
+rewrite IHvars. unfold map_remove.
+rewrite Map.remove_ok.
+destruct (string_dec name (snd head)) as [E|NE];
+  destruct (string_dec (snd head) name) as [E'|NE'];
+  destruct (ListSet.set_mem string_dec name (map snd vars));
+  try easy;
+  try symmetry in E; try contradiction;
+  try symmetry in E'; try contradiction.
+Qed.
+
+Lemma local_vars_agree_erase_unbind {C: VyperConfig}
+                                    (loc40: memory)
+                                    (loc50: string_map dynamic_value)
+                                    (vars: list L50.AST.typename)
+                                    (varcap: N)
+    (Ok: LocalVarsAgree loc40 (L50.LocalVars.unbind_vars vars loc50) varcap):
+  LocalVarsAgree loc40 loc50 varcap.
+Proof.
+intros k L.
+assert (OkK := Ok k L).
+rewrite lookup_unbind in OkK.
+destruct (ListSet.set_mem string_dec (make_var_name "var" k) (map snd vars)).
+{ discriminate. }
+exact OkK.
+Qed.
+
+Lemma stmt_results_agree_erase_unbind {C: VyperConfig}
+                                      (w40 w50: world_state)
+                                      (loc40: memory)
+                                      (loc50: string_map dynamic_value)
+                                      (result40: option (stmt_result uint256))
+                                      (result50: option (stmt_result (list dynamic_value)))
+                                      (vars: list L50.AST.typename)
+                                      (varcap: N)
+   (Ok: StmtResultsAgree (w40, loc40, result40)
+                         (w50, L50.LocalVars.unbind_vars vars loc50, result50)
+                         varcap):
+  StmtResultsAgree (w40, loc40, result40) (w50, loc50, result50) varcap.
+Proof.
+unfold StmtResultsAgree in *.
+split. 2:tauto.
+destruct Ok as (Ok, _).
+apply local_vars_agree_erase_unbind in Ok.
+exact Ok.
+Qed.
+
+
+Lemma translated_stmt_declares_nothing  {C: VyperConfig}
+                                        {B: builtin_names_config}
+                                        {loop_depth: N}
+                                        {protos: string_map proto}
+                                        {s40: L40.AST.stmt}
+                                        {s50: list L50.AST.stmt}
+                                        {this_fun_decl50: option L50.AST.fun_decl}
+                                        (Ok: translate_stmt (match this_fun_decl50 with
+                                                             | Some _ => true
+                                                             | None => false
+                                                             end) B protos s40 loop_depth = inr s50):
+  stmt_list_has_top_level_var_decls s50 = false.
+Proof.
+destruct s40; cbn in Ok.
+{ (* small *)
+  destruct ss; cbn in Ok;
+    try (destruct translate_expr as [|(e', n)]; [| destruct n as [|p]]);
+    try destruct p;
+    try (inversion Ok; subst);
+    try easy;
+    try (destruct ab; cbn in Ok; inversion Ok; now subst);
+    try destruct this_fun_decl50;
+    inversion Ok; subst; easy.
+}
+{ (* switch *)
+  destruct (_ cases) as [err | cases']. { easy. }
+  destruct default as [default|].
+  {
+    destruct translate_block as [err | default']. { easy. }
+    destruct translate_expr as [|(e', n)]; [| destruct n as [|p]];
+      try easy.
+    { inversion Ok; now subst. }
+    destruct p; try easy. inversion Ok; now subst.
+  }
+  destruct translate_expr as [|(e', n)]; [| destruct n as [|p]];
+    try easy.
+  { inversion Ok; now subst. }
+  destruct p; try easy. inversion Ok; now subst.
+}
+(* loop *)
+destruct translate_block as [err | body']. { easy. }
+inversion Ok. now subst.
+Qed.
+
+
+Lemma translated_block_declares_nothing  {C: VyperConfig}
+                                         {B: builtin_names_config}
+                                         {loop_depth: N}
+                                         {protos: string_map proto}
+                                         {b40: L40.AST.block}
+                                         {b50: L50.AST.block}
+                                         {this_fun_decl50: option L50.AST.fun_decl}
+                                         (Ok: translate_block (match this_fun_decl50 with
+                                                               | Some _ => true
+                                                               | None => false
+                                                               end) B protos b40 loop_depth = inr b50):
+  let '(L50.AST.Block s50) := b50 in
+  stmt_list_has_top_level_var_decls s50 = false.
+Proof.
+destruct b40 as (s40).
+destruct b50 as (s50).
+revert s50 Ok. induction s40 as [|head40]; intros; cbn in Ok. { now inversion Ok. }
+remember (translate_stmt match this_fun_decl50 with
+                         | Some _ => true
+                         | None => false
+                         end B protos head40 loop_depth) as head'.
+destruct head' as [|head50]. discriminate. symmetry in Heqhead'.
+cbn in Ok. cbn in IHs40.
+remember (_ s40) as tail50.
+destruct tail50 as [|tail50]. 1:easy.
+inversion Ok; subst.
+rewrite stmt_list_has_top_level_var_decls_app.
+rewrite (translated_stmt_declares_nothing Heqhead').
+now rewrite (IHs40 tail50 eq_refl).
+Qed.
+
+(* to Arith2 *)
+Lemma max_lub_lt_l {a b c : N} (H: (N.max a b < c)%N):
+  (a < c)%N.
+Proof. exact (proj1 (proj1 (N.max_lub_lt_iff _ _ _) H)). Qed.
+Lemma max_lub_lt_r {a b c : N} (H: (N.max a b < c)%N):
+  (b < c)%N.
+Proof. exact (proj2 (proj1 (N.max_lub_lt_iff _ _ _) H)). Qed.
+
+(** Blocks are interpreted correctly provided that statements are interpreted correctly. *)
+Local Lemma interpret_translated_block_weak
+    {C: VyperConfig}
+    {B: builtin_names_config}
+    {protos: string_map proto}
+    {loop_depth: N}
+    {max_loop_iterations: nat}
+    (call40: forall
+                  (decl: L40.AST.decl)
+                  (world: world_state)
+                  (arg_values: list uint256),
+                world_state * option (expr_result uint256))
+    (call50: forall
+                  (decl: L50.AST.fun_decl)
+                  (world: world_state)
+                  (arg_values: list dynamic_value),
+                world_state * option (expr_result (list dynamic_value)))
+    (CallsOk: forall (decl40: L40.AST.decl)
+                     (decl50: L50.AST.fun_decl)
+                     (Ok: translate_fun_decl B protos decl40 = inr decl50)
+                     (world: world_state)
+                     (args40: list uint256)
+                     (args50: list dynamic_value)
+                     (ArgsOk: args50 = map (fun x : uint256 => existT (fun t : yul_type => yul_value t) U256 (yul_uint256 x)) args40),
+                 ResultsAgree (call40 decl40 world args40)
+                              (call50 decl50 world args50) 1%N)
+    (decls40: string_map L40.AST.decl)
+    (decls50: string_map L50.AST.fun_decl)
+    (this_fun_decl40: option L40.AST.decl)
+    (this_fun_decl50: option L50.AST.fun_decl)
+    (FunDeclOk: match this_fun_decl40, this_fun_decl50 with
+                | Some d40, Some d50 =>
+                    translate_fun_decl B protos d40 = inr d50
+                | None, None => True
+                | _, _ => False
+                end)
+    (DeclsOk: translate_fun_decls B protos decls40 = inr decls50)
+    (builtins40: string -> option builtin)
+    (builtins50: string -> option L50.Builtins.yul_builtin)
+    (BuiltinsOk: AllBuiltinsAgreeIfU256 builtins40 builtins50)
+    (BuiltinsBasics: BuiltinsSupportBasics builtins50)
+    (BuiltinsSafe: forall x,
+                     builtins50 ("$" ++ x)%string = None)
+    (ProtosOk: ProtosAgree (map_lookup protos) builtins50)
+    (world: world_state)
+    (loc40: memory)
+    (loc50: string_map dynamic_value)
+    (loop_info: list L40.Expr.loop_ctx)
+    (LoopDepthOk: length loop_info = N.to_nat loop_depth)
+    (SV: SecondaryVarsOk loop_info loc50)
+    (b40: L40.AST.block)
+    (b50: L50.AST.block)
+    (Ok: translate_block (match this_fun_decl50 with
+                          | Some _ => true
+                          | None => false
+                          end) B protos b40 loop_depth = inr b50)
+    (varcap: N)
+    (VarcapOk: (L40.AST.var_cap_block b40 <= varcap)%N)
+    (LocalVarsOk: LocalVarsAgree loc40 loc50 varcap)
+    (EnoughIterations:
+      (L40.AST.max_loop_count_block b40 < N.of_nat max_loop_iterations)%N)
+    (OkB: match b40 with
+          | L40.AST.Block body =>
+             Forall
+               (fun s : L40.AST.stmt =>
+                (AST.var_cap_stmt s <= varcap)%N ->
+                (AST.max_loop_count_stmt s < N.of_nat max_loop_iterations)%N ->
+                forall (loop_depth : N) (s50 : list AST.stmt),
+                translate_stmt match this_fun_decl50 with
+                               | Some _ => true
+                               | None => false
+                               end B protos s loop_depth = inr s50 ->
+                forall (world : world_state) (loc40 : memory) (loc50 : string_map dynamic_value),
+                LocalVarsAgree loc40 loc50 varcap ->
+                forall loop_info : list Expr.loop_ctx,
+                Datatypes.length loop_info = N.to_nat loop_depth ->
+                SecondaryVarsOk loop_info loc50 ->
+                let '(w, l, result) := interpret_stmt_list max_loop_iterations builtins50 (map_lookup decls50)
+                                                           this_fun_decl50 call50
+                                                            world loc50 s50 in
+                StmtResultsAgree
+                  (interpret_stmt_metered decls40 call40 builtins40 world loc40 loop_info s)
+                  (w, l, result)
+                  varcap
+                 /\
+                SecondaryVarsOk loop_info l)
+               body
+      end):
+  let '(L50.AST.Block body50) := b50 in
+  let '(w, l, result) := interpret_stmt_list max_loop_iterations builtins50 
+                                             (map_lookup decls50) this_fun_decl50
+                                             call50 world loc50 body50 in
+  StmtResultsAgree
+    (interpret_block_metered decls40 call40 builtins40 world loc40 loop_info b40)
+    (w, l, result)
+    varcap
+   /\
+  SecondaryVarsOk loop_info l.
+Proof.
+destruct b40 as (s40). destruct b50 as (s50).
+revert world loc40 loc50 s50 Ok LocalVarsOk SV.
+induction s40 as [|head40]; intros; cbn in Ok.
+{ (* base *) inversion Ok. subst s50. clear Ok. cbn. cbn in LocalVarsOk. tauto. }
+remember (translate_stmt _ B protos head40 loop_depth) as head'.
+destruct head' as [|head50]. { discriminate. } symmetry in Heqhead'.
+remember ((fix translate_stmt_list (l : list L40.AST.stmt) : string + list AST.stmt := _) s40) as tail'.
+destruct tail' as [|tail50]. { discriminate. }
+inversion Ok. subst s50. clear Ok. cbn.
+cbn in EnoughIterations. cbn in LocalVarsOk.
+assert (T: translate_block (match this_fun_decl50 with
+                            | Some _ => true
+                            | None => false
+                            end) B protos (L40.AST.Block s40) loop_depth 
+            =
+           inr (L50.AST.Block tail50)).
+{ cbn. now rewrite<- Heqtail'. }
+rewrite interpret_stmt_list_app.
+2: apply (translated_stmt_declares_nothing Heqhead').
+2:{
+  apply (translated_block_declares_nothing T).
+}
+cbn in VarcapOk.
+
+assert (OkHead := Forall_inv OkB (N.max_lub_l _ _ _ VarcapOk) (max_lub_lt_l EnoughIterations)
+                             loop_depth head50 Heqhead'
+                             world loc40 loc50
+                             LocalVarsOk
+                             loop_info LoopDepthOk SV).
+(*
+assert (OkHead := Forall_inv OkB (N.max_lub_l _ _ _ VarcapOk)
+                             (N.max_lub_l _ _ _ EnoughIterations) head50 Heqhead'
+                             world loc40 loc50
+                             (local_vars_agree_weaken_left (local_vars_agree_weaken VarcapOk LocalVarsOk))
+                             ResultDeclared loop_info LoopDepthOk OffsetsOk CursorsOk).
+*)
+destruct (interpret_stmt_metered decls40 call40 builtins40 world loc40 loop_info head40)
+  as ((w', loc40'), result40).
+destruct (interpret_stmt_list max_loop_iterations builtins50 (map_lookup decls50) 
+              this_fun_decl50 call50 world loc50 head50)
+  as ((w50', loc50'), result50).
+destruct result40 as [result40|], result50 as [result50|]; cbn in OkHead; try easy.
+destruct result40, result50; try easy.
+2:{ now destruct a. }
+destruct OkHead as ((LocalVarsOk', W), SV').
+subst w50'.
+assert (X := IHs40 (N.max_lub_r _ _ _ VarcapOk)
+                   (max_lub_lt_r EnoughIterations)
+                   (Forall_inv_tail OkB)
+                   w' loc40' loc50' tail50 T LocalVarsOk'
+                   SV').
+destruct (interpret_stmt_list max_loop_iterations builtins50 (map_lookup decls50) this_fun_decl50 call50 w' loc50' tail50)
+  as ((world'', loc''), result'').
+apply X.
+Qed.
+
+(** A separate lemma for switches because of many different ways switches can go
+    (with/without default, with 0 or 1 value).
+    This lemma starts with the value to switch on being already known.
+    This is straightforward because switches work in exactly the same way in L40 and L50.
+ *)
+
+Local Lemma interpret_translated_switch
+    {C: VyperConfig}
+    {B: builtin_names_config}
+    {protos: string_map proto}
+    {loop_depth: N}
+    {max_loop_iterations: nat}
+    (call40: forall
+                  (decl: L40.AST.decl)
+                  (world: world_state)
+                  (arg_values: list uint256),
+                world_state * option (expr_result uint256))
+    (call50: forall
+                  (decl: L50.AST.fun_decl)
+                  (world: world_state)
+                  (arg_values: list dynamic_value),
+                world_state * option (expr_result (list dynamic_value)))
+    (CallsOk: forall (decl40: L40.AST.decl)
+                     (decl50: L50.AST.fun_decl)
+                     (Ok: translate_fun_decl B protos decl40 = inr decl50)
+                     (world: world_state)
+                     (args40: list uint256)
+                     (args50: list dynamic_value)
+                     (ArgsOk: args50 = map (fun x : uint256 => existT (fun t : yul_type => yul_value t) U256 (yul_uint256 x)) args40),
+                 ResultsAgree (call40 decl40 world args40)
+                              (call50 decl50 world args50) 1%N)
+    (decls40: string_map L40.AST.decl)
+    (decls50: string_map L50.AST.fun_decl)
+    (this_fun_decl40: option L40.AST.decl)
+    (this_fun_decl50: option L50.AST.fun_decl)
+    (FunDeclOk: match this_fun_decl40, this_fun_decl50 with
+                | Some d40, Some d50 =>
+                    translate_fun_decl B protos d40 = inr d50
+                | None, None => True
+                | _, _ => False
+                end)
+    (DeclsOk: translate_fun_decls B protos decls40 = inr decls50)
+    (builtins40: string -> option builtin)
+    (builtins50: string -> option L50.Builtins.yul_builtin)
+    (BuiltinsOk: AllBuiltinsAgreeIfU256 builtins40 builtins50)
+    (BuiltinsBasics: BuiltinsSupportBasics builtins50)
+    (BuiltinsSafe: forall x,
+                     builtins50 ("$" ++ x)%string = None)
+    (ProtosOk: ProtosAgree (map_lookup protos) builtins50)
+    (world: world_state)
+    (loc40: memory)
+    (loc50: string_map dynamic_value)
+    (loop_info: list L40.Expr.loop_ctx)
+    (LoopDepthOk: length loop_info = N.to_nat loop_depth)
+    (SV: SecondaryVarsOk loop_info loc50)
+    (cases40: list L40.AST.case)
+    (cases50: list L50.AST.case)
+    (OkCases:  (fix translate_cases (l: list L40.AST.case): string + list AST.case :=
+                   match l with
+                   | nil => inr nil
+                   | L40.AST.Case guard body :: t =>
+                       match
+                         translate_block match this_fun_decl50 with
+                                         | Some _ => true
+                                         | None => false
+                                         end B protos body loop_depth
+                       with
+                       | inl err => inl err
+                       | inr body' =>
+                           match translate_cases t with
+                           | inl err => inl err
+                           | inr t' => inr (AST.Case U256 (yul_uint256 guard) body' :: t')
+                           end
+                       end
+                   end) cases40 = inr cases50)
+    (default40: option L40.AST.block)
+    (default50: option L50.AST.block)
+    (OkDefault:
+      match default40, default50 with
+      | None, None => True
+      | Some d40, Some d50 => translate_block match this_fun_decl50 with
+                                              | Some _ => true
+                                              | None => false
+                                              end B protos d40 loop_depth = inr d50
+      | _, _ => False
+      end)
+    (varcap: N)
+    (VarcapOk: ((N.max
+                 ((fix var_cap_cases (l : list L40.AST.case) : N :=
+                     match l with
+                     | nil => 0
+                     | L40.AST.Case _ body :: t => N.max (AST.var_cap_block body) (var_cap_cases t)
+                     end) cases40) 
+                 (match default40 with
+                  | None => 0%N
+                  | Some d => L40.AST.var_cap_block d
+                  end)) <= varcap)%N)
+    (LocalVarsOk: LocalVarsAgree loc40 loc50 varcap)
+    (EnoughIterations:
+      (let
+        fix max_loop_count_cases (l : list L40.AST.case) : N :=
+          match l with
+          | nil => 0%N
+          | L40.AST.Case _ body :: t => N.max (L40.AST.max_loop_count_block body)
+                                              (max_loop_count_cases t)
+          end in
+        let d := match default40 with
+               | Some b => L40.AST.max_loop_count_block b
+               | None => 0%N
+               end in
+      N.max (max_loop_count_cases cases40) d <
+        N.of_nat max_loop_iterations)%N)
+    (CasesWork: Forall
+                  (fun case: L40.AST.case =>
+                   match case with
+                   | L40.AST.Case _ (L40.AST.Block body) =>
+                       Forall
+                         (fun s : L40.AST.stmt =>
+                          (AST.var_cap_stmt s <= varcap)%N ->
+                          (AST.max_loop_count_stmt s < N.of_nat max_loop_iterations)%N ->
+                          forall (loop_depth : N) (s50 : list AST.stmt),
+                          translate_stmt match this_fun_decl50 with
+                                         | Some _ => true
+                                         | None => false
+                                         end B protos s loop_depth = inr s50 ->
+                          forall (world : world_state) (loc40 : memory) (loc50 : string_map dynamic_value),
+                          LocalVarsAgree loc40 loc50 varcap ->
+                          forall loop_info : list Expr.loop_ctx,
+                          Datatypes.length loop_info = N.to_nat loop_depth ->
+                          SecondaryVarsOk loop_info loc50 ->
+                          let
+                          '(w, l, result) :=
+                           interpret_stmt_list max_loop_iterations builtins50 (map_lookup decls50) this_fun_decl50 call50
+                             world loc50 s50 in
+                           StmtResultsAgree (interpret_stmt_metered decls40 call40 builtins40 world loc40 loop_info s)
+                             (w, l, result) varcap /\
+                           SecondaryVarsOk loop_info l) body
+                   end) cases40)
+    (DefaultWorks: match default40 with
+                   | Some (L40.AST.Block d) =>
+                       Forall
+                         (fun s : L40.AST.stmt =>
+                          (AST.var_cap_stmt s <= varcap)%N ->
+                          (AST.max_loop_count_stmt s < N.of_nat max_loop_iterations)%N ->
+                          forall (loop_depth : N) (s50 : list AST.stmt),
+                          translate_stmt match this_fun_decl50 with
+                                         | Some _ => true
+                                         | None => false
+                                         end B protos s loop_depth = inr s50 ->
+                          forall (world : world_state) (loc40 : memory) (loc50 : string_map dynamic_value),
+                          LocalVarsAgree loc40 loc50 varcap  ->
+                          forall loop_info : list Expr.loop_ctx,
+                          Datatypes.length loop_info = N.to_nat loop_depth ->
+                          SecondaryVarsOk loop_info loc50 ->
+                          let
+                          '(w, l, result) :=
+                           interpret_stmt_list max_loop_iterations builtins50 (map_lookup decls50) this_fun_decl50 call50
+                             world loc50 s50 in
+                           StmtResultsAgree (interpret_stmt_metered decls40 call40 builtins40 world loc40 loop_info s)
+                             (w, l, result) varcap /\
+                           SecondaryVarsOk loop_info l)
+                         d
+                    | None => True
+                    end)
+    (value: uint256):
+  let fix dispatch50 (l: list L50.AST.case)
+       : world_state * string_map dynamic_value * option (stmt_result (list dynamic_value))
+       := match l with
+          | (L50.AST.Case guard_type guard body) :: tail =>
+              if yul_type_eq_dec U256 guard_type
+                then if (Z_of_uint256 value
+                          =?
+                         Z_of_uint256 (uint256_of_yul_value guard))%Z
+                        then L50.Stmt.interpret_block max_loop_iterations
+                                                      builtins50 (map_lookup decls50) this_fun_decl50 call50
+                                                      world loc50 nop body
+                        else dispatch50 tail
+                else (world, loc50, Some (stmt_error (L50.DynError.string_of_dynamic_error
+                                                      (L50.DynError.DE_TypeMismatch guard_type U256))))
+          | nil =>
+                   match default50 with
+                   | Some body =>
+                        L50.Stmt.interpret_block max_loop_iterations
+                                                 builtins50 (map_lookup decls50) this_fun_decl50 call50
+                                                 world loc50 nop body
+                   | None => (world, loc50, Some StmtSuccess)
+                   end
+          end in
+  let '(w, l, result) := dispatch50 cases50 in
+  StmtResultsAgree
+    (let fix dispatch40 (l: list L40.AST.case)
+         : world_state * memory * option (stmt_result uint256)
+         := match l with
+            | cons (L40.AST.Case guard block) t =>
+                if (Z_of_uint256 value =? Z_of_uint256 guard)%Z
+                  then interpret_block_metered decls40 call40 builtins40
+                                               world loc40 loop_info block
+                  else dispatch40 t
+            | nil => match default40 with
+                     | Some block =>
+                          interpret_block_metered decls40 call40 builtins40
+                                                  world loc40 loop_info block
+                     | None => (world, loc40, Some StmtSuccess)
+                     end
+            end
+     in dispatch40 cases40)
+    (w, l, result)
+    varcap
+     /\
+    SecondaryVarsOk loop_info l.
+Proof.
+revert cases50 OkCases. induction cases40 as [|head]; intros.
+{
+  inversion OkCases. subst cases50. cbn.
+  destruct default40 as [d40|], default50 as [d50|]; try easy.
+  destruct d50 as (d50). rewrite interpret_stmt_list_ok.
+  apply (interpret_translated_block_weak call40 call50 CallsOk decls40 decls50
+                                         this_fun_decl40 this_fun_decl50 FunDeclOk
+                                         DeclsOk builtins40 builtins50 BuiltinsOk
+                                         BuiltinsBasics BuiltinsSafe ProtosOk
+                                         world loc40 loc50
+                                         loop_info LoopDepthOk SV
+                                         d40 (L50.AST.Block d50) OkDefault varcap (N.max_lub_r _ _ _ VarcapOk)
+                                         LocalVarsOk (max_lub_lt_r EnoughIterations) DefaultWorks).
+}
+destruct head as (guard, body).
+remember (translate_block match this_fun_decl50 with
+                          | Some _ => true
+                          | None => false
+                          end B protos body loop_depth) as head'.
+destruct head' as [|head50]. { discriminate. }
+remember ((fix translate_cases (l : list L40.AST.case) : string + list AST.case := _) cases40) as tail'.
+destruct tail' as [|tail50]. { discriminate. }
+inversion OkCases; subst cases50; clear OkCases.
+cbn.
+destruct (Z_of_uint256 value =? Z_of_uint256 guard)%Z.
+{ (* taking the case *)
+  destruct head50 as (head50). rewrite interpret_stmt_list_ok.
+  apply (interpret_translated_block_weak call40 call50 CallsOk decls40 decls50
+                                         this_fun_decl40 this_fun_decl50 FunDeclOk
+                                         DeclsOk builtins40 builtins50 BuiltinsOk
+                                         BuiltinsBasics BuiltinsSafe ProtosOk
+                                         world loc40 loc50
+                                         loop_info LoopDepthOk SV
+                                         body (L50.AST.Block head50) (eq_sym Heqhead')
+                                         varcap (N.max_lub_l _ _ _  (N.max_lub_l _ _ _ VarcapOk))
+                                         LocalVarsOk (max_lub_lt_l (max_lub_lt_l EnoughIterations))
+                                         (Forall_inv CasesWork)).
+}
+(* not taking the case *)
+cbn in EnoughIterations.
+apply (IHcases40 (N.max_lub _ _ _ (N.max_lub_r _ _ _  (N.max_lub_l _ _ _ VarcapOk))
+                                  (N.max_lub_r _ _ _ VarcapOk))
+                 (N.max_lub_lt _ _ _ (max_lub_lt_r (max_lub_lt_l EnoughIterations))
+                                     (max_lub_lt_r EnoughIterations))
+                 (Forall_inv_tail CasesWork)
+                 tail50 eq_refl).
+Qed.
+
+Lemma interpret_translated_stmt {C: VyperConfig}
+                                {B: builtin_names_config}
+                                {protos: string_map proto}
+                                {s40: L40.AST.stmt}
+                                {s50: list L50.AST.stmt}
+                                {loop_depth: N}
+                                {max_loop_iterations: nat}
+                                (call40: forall
+                                              (decl: L40.AST.decl)
+                                              (world: world_state)
+                                              (arg_values: list uint256),
+                                            world_state * option (expr_result uint256))
+                                (call50: forall
+                                              (decl: L50.AST.fun_decl)
+                                              (world: world_state)
+                                              (arg_values: list dynamic_value),
+                                            world_state * option (expr_result (list dynamic_value)))
+                                (CallsOk: forall (decl40: L40.AST.decl)
+                                                 (decl50: L50.AST.fun_decl)
+                                                 (Ok: translate_fun_decl B protos decl40 = inr decl50)
+                                                 (world: world_state)
+                                                 (args40: list uint256)
+                                                 (args50: list dynamic_value)
+                                                 (ArgsOk: args50 = map (fun x : uint256 => existT (fun t : yul_type => yul_value t) U256 (yul_uint256 x)) args40),
+                                             ResultsAgree (call40 decl40 world args40)
+                                                          (call50 decl50 world args50) 1%N)
+                                (decls40: string_map L40.AST.decl)
+                                (decls50: string_map L50.AST.fun_decl)
+                                (this_fun_decl40: option L40.AST.decl)
+                                (this_fun_decl50: option L50.AST.fun_decl)
+                                (FunDeclOk: match this_fun_decl40, this_fun_decl50 with
+                                            | Some d40, Some d50 =>
+                                                translate_fun_decl B protos d40 = inr d50
+                                            | None, None => True
+                                            | _, _ => False
+                                            end)
+                                (Ok: translate_stmt (match this_fun_decl50 with
+                                                     | Some _ => true
+                                                     | None => false
+                                                     end) B protos s40 loop_depth = inr s50)
+                                (DeclsOk: translate_fun_decls B protos decls40 = inr decls50)
+                                (builtins40: string -> option builtin)
+                                (builtins50: string -> option L50.Builtins.yul_builtin)
+                                (BuiltinsOk: AllBuiltinsAgreeIfU256 builtins40 builtins50)
+                                (BuiltinsBasics: BuiltinsSupportBasics builtins50)
+                                (BuiltinsSafe: forall x,
+                                                 builtins50 ("$" ++ x)%string = None)
+                                (BuiltinsHaveArith: BuiltinsSupportUInt256 B builtins40)
+                                (ProtosOk: ProtosAgree (map_lookup protos) builtins50)
+                                (KnownProtosOk: check_known_protos B (map_lookup protos) = true)
+                                (world: world_state)
+                                (loc40: memory)
+                                (loc50: string_map dynamic_value)
+                                (varcap: N)
+                                (VarcapOk: (L40.AST.var_cap_stmt s40 <= varcap)%N)
+                                (EnoughIterations:
+                                  (L40.AST.max_loop_count_stmt s40 < N.of_nat max_loop_iterations)%N)
+                                (LocalVarsOk: LocalVarsAgree loc40 loc50 varcap)
+                                (loop_info: list L40.Expr.loop_ctx)
+                                (LoopDepthOk: length loop_info = N.to_nat loop_depth)
+                                (SV: SecondaryVarsOk loop_info loc50):
+  let '(w, l, result) := L50.Stmt.interpret_stmt_list max_loop_iterations builtins50
+                                                      (map_lookup decls50)
+                                                      this_fun_decl50 call50
+                                                      world loc50 s50
+  in
+  StmtResultsAgree
+    (interpret_stmt_metered decls40 call40 builtins40 world loc40 loop_info s40)
+    (w, l, result)
+    varcap
+   /\
+  SecondaryVarsOk loop_info l.
+Proof.
+revert loop_depth s50 Ok world loc40 loc50 LocalVarsOk loop_info LoopDepthOk SV.
+induction s40 using L40.AST.stmt_ind'; intros.
+{ (* small stmt *)
+  apply (interpret_translated_small_stmt call40 call50 CallsOk decls40 decls50
+                                         this_fun_decl40 this_fun_decl50 FunDeclOk Ok DeclsOk
+                                         builtins40 builtins50 BuiltinsOk BuiltinsBasics BuiltinsSafe
+                                         ProtosOk world loc40 loc50 varcap VarcapOk LocalVarsOk
+                                         loop_info
+                                         LoopDepthOk SV).
+}
+{ (* switch without default *)
+  cbn in Ok.
+  remember (translate_expr protos e loop_depth) as e'. symmetry in Heqe'.
+  destruct e' as [|(e', n)]. { now destruct (_ cases). }
+  cbn in LocalVarsOk, VarcapOk.
+  assert (ValueOk := interpret_translated_expr Heqe' call40 call50 CallsOk decls40 decls50 DeclsOk
+                                               builtins40 builtins50 BuiltinsOk BuiltinsSafe
+                                               ProtosOk world loc40 loc50
+                                               (local_vars_agree_weaken_left
+                                                 (local_vars_agree_weaken VarcapOk LocalVarsOk))
+                                               loop_info LoopDepthOk 
+                                               (sv_offsets_agree SV) (sv_cursors_agree SV)).
+  unfold ResultsAgree in ValueOk.
+  remember ((fix translate_cases (l : list L40.AST.case) : string + list AST.case := _) cases) as cases'.
+  destruct cases' as [|cases50]. { discriminate. }
+  destruct n as [|p].
+  { (* 0 values *)
+    inversion Ok. subst s50. clear Ok.
+
+    (* dance around cbn's horrors *)
+    cbn delta iota.
+    unfold L50.Stmt.interpret_stmt_list.
+    cbn delta iota.
+    remember (L50.DynError.string_of_dynamic_error) as stringify.
+    remember yul_type_eq_dec as yt_eq.
+    cbn.
+
+    destruct (interpret_expr_metered decls40 call40 builtins40 world loc40 loop_info e) as (w40, r40).
+    destruct (interpret_expr builtins50 (map_lookup decls50) call50 world loc50 e') as (w50, r50).
+    destruct ValueOk as (W, ValueOk). subst w40.
+    destruct r40 as [r40|], r50 as [r50|]; try easy.
+    destruct r40 as [val40|ab40], r50 as [val50|ab50]; try easy.
+    destruct val50. 2:{ cbn in ValueOk. now destruct val50. }
+    assert (X := interpret_translated_switch call40 call50 CallsOk decls40 decls50
+                                             this_fun_decl40 this_fun_decl50 FunDeclOk
+                                             DeclsOk builtins40 builtins50 BuiltinsOk
+                                             BuiltinsBasics BuiltinsSafe ProtosOk
+                                             w50 loc40 loc50
+                                             loop_info LoopDepthOk SV
+                                             cases cases50 (eq_sym Heqcases')
+                                             None None I
+                                             varcap (N.max_lub_r _ _ _ VarcapOk)
+                                             LocalVarsOk EnoughIterations H I val40).
+    rewrite<- Heqstringify in X.
+    rewrite<- Heqyt_eq in X.
+    cbn in X.
+    cbn in ValueOk. destruct ValueOk as (V, _). subst val40.
+    destruct ((fix dispatch50 (l : list L50.AST.case) := _) cases50) as ((ww50, l50), result50).
+    destruct (((fix dispatch40 (l : list L40.AST.case) : world_state * memory * option (stmt_result uint256) :=
+          match l with
+          | nil => (w50, loc40, Some StmtSuccess)
+          | L40.AST.Case guard block :: t =>
+              if (Z_of_uint256 zero256 =? Z_of_uint256 guard)%Z
+              then interpret_block_metered decls40 call40 builtins40 w50 loc40 loop_info block
+              else dispatch40 t
+          end) cases)) as ((w40, l40), result40).
+    destruct result50 as [result50|]. 2:tauto. { now destruct result50. }
+    cbn in ValueOk. subst ab40. now destruct ab50.
+  }
+  (* 1 value *)
+  destruct p; try discriminate.
+  inversion Ok. subst s50. clear Ok.
+
+  (* dance around cbn's horrors *)
+  cbn delta iota.
+  unfold L50.Stmt.interpret_stmt_list.
+  cbn delta iota.
+  remember (L50.DynError.string_of_dynamic_error) as stringify.
+  remember yul_type_eq_dec as yt_eq.
+  cbn.
+
+  destruct (interpret_expr_metered decls40 call40 builtins40 world loc40 loop_info e) as (w40, r40).
+  destruct (interpret_expr builtins50 (map_lookup decls50) call50 world loc50 e') as (w50, r50).
+  destruct ValueOk as (W, ValueOk). subst w40.
+  destruct r40 as [r40|], r50 as [r50|]; try easy.
+  destruct r40 as [val40|ab40], r50 as [val50|ab50]; try easy.
+  2:{ cbn in ValueOk. subst ab40. now destruct ab50. }
+
+  unfold ExprResultsAgree in ValueOk.
+  destruct val50 as [|val50]. { cbn in ValueOk. assert (Bad: 1%N = 0%N) by tauto. discriminate. }
+  destruct val0 (* how to rename it? *). 2:contradiction.
+  destruct ValueOk as (V, _). subst val50.
+  assert (X := interpret_translated_switch call40 call50 CallsOk decls40 decls50
+                                           this_fun_decl40 this_fun_decl50 FunDeclOk
+                                           DeclsOk builtins40 builtins50 BuiltinsOk
+                                           BuiltinsBasics BuiltinsSafe ProtosOk
+                                           w50 loc40 loc50
+                                           loop_info LoopDepthOk SV
+                                           cases cases50 (eq_sym Heqcases')
+                                           None None I
+                                           varcap (N.max_lub_r _ _ _ VarcapOk)
+                                           LocalVarsOk EnoughIterations H I val40).
+  rewrite<- Heqstringify in X.
+  rewrite<- Heqyt_eq in X.
+  cbn in X.
+  destruct ((fix dispatch50 (l : list L50.AST.case) := _) cases50) as ((ww50, l50), result50).
+  destruct (((fix dispatch40 (l : list L40.AST.case) : world_state * memory * option (stmt_result uint256) :=
+        match l with
+        | nil => (w50, loc40, Some StmtSuccess)
+        | L40.AST.Case guard block :: t =>
+            if (Z_of_uint256 zero256 =? Z_of_uint256 guard)%Z
+            then interpret_block_metered decls40 call40 builtins40 w50 loc40 loop_info block
+            else dispatch40 t
+        end) cases)) as ((w40, l40), result40).
+  destruct result50 as [result50|]. 2:tauto. now destruct result50.
+}
+{ (* switch with default (of course massive dup) *)
+  cbn in Ok.
+  remember (translate_expr protos e loop_depth) as e'. symmetry in Heqe'.
+  destruct e' as [|(e', n)].
+  {
+    destruct (_ cases) as [|cases']. { discriminate. }
+    now destruct (_ default).
+  }
+  cbn in LocalVarsOk, VarcapOk.
+  assert (ValueOk := interpret_translated_expr Heqe' call40 call50 CallsOk decls40 decls50 DeclsOk
+                                               builtins40 builtins50 BuiltinsOk BuiltinsSafe
+                                               ProtosOk world loc40 loc50
+                                               (local_vars_agree_weaken_left
+                                                 (local_vars_agree_weaken VarcapOk LocalVarsOk))
+                                               loop_info LoopDepthOk
+                                               (sv_offsets_agree SV) (sv_cursors_agree SV)).
+  unfold ResultsAgree in ValueOk.
+  remember ((fix translate_cases (l : list L40.AST.case) : string + list AST.case := _) cases)
+    as cases'.
+  destruct cases' as [|cases50]. { discriminate. }
+  remember ((fix translate_stmt_list (l : list L40.AST.stmt) : string + list AST.stmt := _) default)
+    as default'.
+  destruct default' as [|default50]. { discriminate. }
+  destruct n as [|p].
+  { (* 0 values *)
+    inversion Ok. subst s50. clear Ok.
+
+    (* dance around cbn's horrors *)
+    cbn delta iota.
+    unfold L50.Stmt.interpret_stmt_list.
+    cbn delta iota.
+    remember (L50.DynError.string_of_dynamic_error) as stringify.
+    remember yul_type_eq_dec as yt_eq.
+    cbn.
+
+    destruct (interpret_expr_metered decls40 call40 builtins40 world loc40 loop_info e) as (w40, r40).
+    destruct (interpret_expr builtins50 (map_lookup decls50) call50 world loc50 e') as (w50, r50).
+    destruct ValueOk as (W, ValueOk). subst w40.
+    destruct r40 as [r40|], r50 as [r50|]; try easy.
+    destruct r40 as [val40|ab40], r50 as [val50|ab50]; try easy.
+    2:{ cbn in ValueOk. subst ab40. now destruct ab50. }
+    destruct val50. 2:{ cbn in ValueOk. now destruct val50. }
+    assert (DefaultsOk: translate_block
+                          match this_fun_decl50 with
+                          | Some _ => true
+                          | None => false
+                          end
+                          B protos (L40.AST.Block default) loop_depth = inr (AST.Block default50)).
+    { cbn. now rewrite<- Heqdefault'. }
+    assert (X := interpret_translated_switch call40 call50 CallsOk decls40 decls50
+                                             this_fun_decl40 this_fun_decl50 FunDeclOk
+                                             DeclsOk builtins40 builtins50 BuiltinsOk
+                                             BuiltinsBasics BuiltinsSafe ProtosOk
+                                             w50 loc40 loc50
+                                             loop_info LoopDepthOk SV
+                                             cases cases50 (eq_sym Heqcases')
+                                             (Some (L40.AST.Block default)) (Some (L50.AST.Block default50))
+                                             DefaultsOk
+                                             varcap (N.max_lub_r _ _ _ VarcapOk)
+                                             LocalVarsOk EnoughIterations H H0 val40).
+    rewrite<- Heqstringify in X.
+    rewrite<- Heqyt_eq in X.
+    cbn in X.
+    cbn in ValueOk. destruct ValueOk as (V, _). subst val40.
+    destruct ((fix dispatch50 (l : list L50.AST.case) := _) cases50) as ((ww50, l50), result50).
+    destruct (((fix dispatch40 (l : list L40.AST.case) : world_state * memory * option (stmt_result uint256) :=
+          match l with
+          | nil => (w50, loc40, Some StmtSuccess)
+          | L40.AST.Case guard block :: t =>
+              if (Z_of_uint256 zero256 =? Z_of_uint256 guard)%Z
+              then interpret_block_metered decls40 call40 builtins40 w50 loc40 loop_info block
+              else dispatch40 t
+          end) cases)) as ((w40, l40), result40).
+    destruct result50 as [result50|]. 2:tauto. now destruct result50.
+  }
+  (* 1 value *)
+  destruct p; try discriminate.
+  inversion Ok. subst s50. clear Ok.
+
+  (* dance around cbn's horrors *)
+  cbn delta iota.
+  unfold L50.Stmt.interpret_stmt_list.
+  cbn delta iota.
+  remember (L50.DynError.string_of_dynamic_error) as stringify.
+  remember yul_type_eq_dec as yt_eq.
+  cbn.
+
+  destruct (interpret_expr_metered decls40 call40 builtins40 world loc40 loop_info e) as (w40, r40).
+  destruct (interpret_expr builtins50 (map_lookup decls50) call50 world loc50 e') as (w50, r50).
+  destruct ValueOk as (W, ValueOk). subst w40.
+  destruct r40 as [r40|], r50 as [r50|]; try easy.
+  destruct r40 as [val40|ab40], r50 as [val50|ab50]; try easy.
+  2:{ cbn in ValueOk. subst ab40. now destruct ab50. }
+
+  unfold ExprResultsAgree in ValueOk.
+  destruct val50 as [|val50]. { cbn in ValueOk. assert (Bad: 1%N = 0%N) by tauto. discriminate. }
+  destruct val0 (* how to rename it? *). 2:contradiction.
+  destruct ValueOk as (V, _). subst val50.
+  assert (DefaultsOk: translate_block
+                        match this_fun_decl50 with
+                        | Some _ => true
+                        | None => false
+                        end
+                        B protos (L40.AST.Block default) loop_depth = inr (AST.Block default50)).
+  { cbn. now rewrite<- Heqdefault'. }
+  assert (X := interpret_translated_switch call40 call50 CallsOk decls40 decls50
+                                           this_fun_decl40 this_fun_decl50 FunDeclOk
+                                           DeclsOk builtins40 builtins50 BuiltinsOk
+                                           BuiltinsBasics BuiltinsSafe ProtosOk
+                                           w50 loc40 loc50
+                                           loop_info LoopDepthOk SV
+                                           cases cases50 (eq_sym Heqcases')
+                                           (Some (L40.AST.Block default)) (Some (L50.AST.Block default50))
+                                           DefaultsOk
+                                           varcap (N.max_lub_r _ _ _ VarcapOk)
+                                           LocalVarsOk EnoughIterations H H0 val40).
+  rewrite<- Heqstringify in X.
+  rewrite<- Heqyt_eq in X.
+  cbn in X.
+  destruct ((fix dispatch50 (l : list L50.AST.case) := _) cases50) as ((ww50, l50), result50).
+  destruct (((fix dispatch40 (l : list L40.AST.case) : world_state * memory * option (stmt_result uint256) :=
+        match l with
+        | nil => (w50, loc40, Some StmtSuccess)
+        | L40.AST.Case guard block :: t =>
+            if (Z_of_uint256 zero256 =? Z_of_uint256 guard)%Z
+            then interpret_block_metered decls40 call40 builtins40 w50 loc40 loop_info block
+            else dispatch40 t
+        end) cases)) as ((w40, l40), result40).
+  destruct result50 as [result50|]. 2:tauto. now destruct result50.
+}
+(********************************** loop **********************************)
+cbn delta iota in Ok.
+remember (make_var_name "var") as var_name. (* prevent cbn horrors *)
+remember (make_var_name "offset") as offset_name.
+remember (make_var_name "cursor") as cursor_name.
+cbn in Ok.
+remember ((fix translate_stmt_list (l : list L40.AST.stmt) : string + list AST.stmt := _) body) as body'.
+destruct body' as [|body50]. { discriminate. }
+inversion Ok. subst s50. clear Ok.
+cbn in EnoughIterations.
+
+(* remembering everything away from cbn *)
+remember (AST.VarDecl ((U256, cursor_name loop_depth) :: nil) None :: nil) as cursor_decl.
+remember ((AST.FunCall (builtin_name_uint256_lt B)
+           (AST.LocVar (cursor_name loop_depth) :: AST.Const U256 (yul_uint256 count) :: nil)))
+  as cond_expr.
+remember (AST.Block
+           (AST.Assign (cursor_name loop_depth :: nil)
+              (AST.FunCall (builtin_name_uint256_add B)
+                 (AST.LocVar (cursor_name loop_depth) :: AST.Const U256 (yul_uint256 one256) :: nil))
+            :: nil))
+  as increment.
+remember (AST.Block body50) as bodyblock50.
+remember (L40.AST.Block body) as bodyblock40.
+cbn. (* it still opens yul_type_eq_dec :( *)
+remember (fix iterate
+            (count0 : nat) (world0 : world_state) (loc : string_map dynamic_value) {struct count0} :
+              world_state * string_map dynamic_value * option (stmt_result (list dynamic_value)) := _)
+  as iterate50.
+remember (fix do_loop (world0 : world_state) (loc : memory) (countdown : nat) {struct countdown} :
+            world_state * memory * option (stmt_result uint256) := _) as iterate40.
+
+(* load the variable with the offset value *)
+cbn in VarcapOk.
+assert (InitVarUnderCap: (var < varcap)%N) by lia.
+assert (InitVarOk := LocalVarsOk var InitVarUnderCap).
+unfold map_lookup in InitVarOk. rewrite<- Heqvar_name in InitVarOk.
+rewrite InitVarOk. cbn.
+
+(* ensure that our offset variable isn't declared yet *)
+assert (OffsetUndeclared := sv_offsets_undeclared SV (N.to_nat loop_depth)
+                                                     (Nat.eq_le_incl _ _ LoopDepthOk)).
+rewrite<-Heqoffset_name in OffsetUndeclared. rewrite N2Nat.id in OffsetUndeclared.
+rewrite OffsetUndeclared.
+
+(* declare cursor *)
+subst cursor_decl. cbn.
+assert (CursorUndeclared := sv_cursors_undeclared SV (N.to_nat loop_depth)
+                                                     (Nat.eq_le_incl _ _ LoopDepthOk)).
+unfold map_lookup in *. unfold map_insert in *.
+rewrite<-Heqcursor_name in CursorUndeclared. rewrite N2Nat.id in CursorUndeclared.
+rewrite Map.insert_ok.
+destruct string_dec. { subst. discriminate. }
+rewrite CursorUndeclared.
+
+(* we obtain the varmap with new offset and cursor variables *)
+remember (@Map.insert string string_dec (@dynamic_value C) (@string_map C (@dynamic_value C))
+             (@string_map_impl C (@dynamic_value C))
+             (@Map.insert string string_dec (@dynamic_value C) (@string_map C (@dynamic_value C))
+                (@string_map_impl C (@dynamic_value C)) loc50 (offset_name loop_depth)
+                (@existT yul_type (fun t : yul_type => @yul_value C t) U256
+                   (@yul_uint256 C
+                      (@OpenArray.get (@uint256 C) (@uint256_of_Z C 0) (@memory C) 
+                         (@memory_impl C) loc40 var)))) (cursor_name loop_depth)
+             (@existT yul_type (fun t : yul_type => @yul_value C t) U256 (@int_zero_value C I256 false)))
+  as current_loc50.
+
+assert (CurrentLocalVarsOk: LocalVarsAgree loc40 current_loc50 varcap).
+{
+  intros k L.
+  subst current_loc50.
+  unfold map_lookup.
+  subst offset_name cursor_name.
+  repeat rewrite Map.insert_ok.
+  destruct string_dec. { discriminate. }
+  destruct string_dec. { discriminate. }
+  apply (LocalVarsOk k L).
+}
+
+assert (CondExprWorks: forall w l cursor,
+         map_lookup l (cursor_name loop_depth) = Some (existT _ U256 (yul_uint256 cursor))
+          ->
+         interpret_expr builtins50 (map_lookup decls50) call50 w l cond_expr
+          =
+         (w, Some (ExprSuccess
+               ((if (Z_of_uint256 cursor <? Z_of_uint256 count)%Z
+                    then existT _ U256 (yul_uint256 one256)
+                    else existT _ U256 (yul_uint256 zero256))
+                  :: nil)))).
+{
+  assert (LtProtoChecked: check_proto (map_lookup protos (builtin_name_uint256_lt B)) 2 1 = true).
+  {
+    unfold check_known_protos in KnownProtosOk.
+    unfold map_lookup.
+    destruct (check_proto (Map.lookup protos (builtin_name_uint256_lt B)) 2 1). { trivial. }
+    repeat rewrite Bool.andb_false_r in KnownProtosOk.
+    repeat rewrite Bool.andb_false_l in KnownProtosOk.
+    discriminate.
+  }
+  unfold BuiltinsSupportUInt256 in BuiltinsHaveArith.
+  assert (LtSupported: BuiltinsSupportBinop builtins40 (builtin_name_uint256_lt B) UInt256.uint256_lt)
+    by tauto.
+  assert (LtSpec := binop_to_yul BuiltinsOk ProtosOk LtProtoChecked LtSupported).
+  intros w l cursor Q.
+  subst cond_expr. cbn.
+  assert (DeclsMangled := translated_decls_start_with_dollar decls40 decls50 DeclsOk (builtin_name_uint256_lt B)).
+  assert (LtNotMangled := proj1 (mangled_safety_equiv builtins50) BuiltinsSafe 
+                                (builtin_name_uint256_lt B)).
+  unfold map_lookup in *.
+  destruct (builtins50 (builtin_name_uint256_lt B)) as [b|]. 2:contradiction.
+  destruct (Map.lookup decls50 (builtin_name_uint256_lt B)).
+  {
+    assert (F: forall {T} (x: T), Some x <> None) by discriminate.
+    assert (M := DeclsMangled (F _ _)).
+    assert (N := LtNotMangled (F _ _)).
+    rewrite M in N. discriminate.
+  }
+  unfold dynamic_value. rewrite Q.
+  cbn. rewrite LtSpec. unfold UInt256.uint256_lt.
+  now destruct (Z_of_uint256 cursor <? Z_of_uint256 count)%Z.
+}
+clear Heqcond_expr.
+
+assert (IncrementWorks: forall w l cursor,
+         map_lookup l (cursor_name loop_depth) = Some (existT _ U256 (yul_uint256 cursor))
+          ->
+         interpret_block max_loop_iterations builtins50 (map_lookup decls50) this_fun_decl50 call50 w l nop increment
+          =
+         (w,
+          map_insert l (cursor_name loop_depth)
+             (existT _ U256 (yul_uint256 (uint256_of_Z (Z_of_uint256 cursor + 1%Z)))),
+          Some StmtSuccess)).
+{
+  assert (AddProtoChecked: check_proto (map_lookup protos (builtin_name_uint256_add B)) 2 1 = true).
+  {
+    unfold check_known_protos in KnownProtosOk.
+    unfold map_lookup.
+    destruct (check_proto (Map.lookup protos (builtin_name_uint256_add B)) 2 1). { trivial. }
+    repeat rewrite Bool.andb_false_r in KnownProtosOk.
+    repeat rewrite Bool.andb_false_l in KnownProtosOk.
+    discriminate.
+  }
+  unfold BuiltinsSupportUInt256 in BuiltinsHaveArith.
+  assert (AddSupported: BuiltinsSupportBinop builtins40 (builtin_name_uint256_add B) CheckedArith.uint256_add)
+    by tauto.  (* XXX: CheckedArith.uint256_add is actually unchecked modulo - needs to be renamed! *)
+  assert (AddSpec := binop_to_yul BuiltinsOk ProtosOk AddProtoChecked AddSupported).
+  intros w l cursor Q.
+  subst increment. cbn.
+  assert (DeclsMangled := translated_decls_start_with_dollar decls40 decls50 DeclsOk (builtin_name_uint256_add B)).
+  assert (AddNotMangled := proj1 (mangled_safety_equiv builtins50) BuiltinsSafe 
+                                 (builtin_name_uint256_add B)).
+  unfold map_lookup in *.
+  destruct (builtins50 (builtin_name_uint256_add B)) as [b|]. 2:contradiction.
+  destruct (Map.lookup decls50 (builtin_name_uint256_add B)).
+  {
+    assert (F: forall {T} (x: T), Some x <> None) by discriminate.
+    assert (M := DeclsMangled (F _ _)).
+    assert (N := AddNotMangled (F _ _)).
+    rewrite M in N. discriminate.
+  }
+  unfold dynamic_value. rewrite Q.
+  cbn. rewrite AddSpec. unfold CheckedArith.uint256_add. cbn.
+  unfold nop. repeat f_equal.
+  unfold one256. now rewrite uint256_ok.
+}
+clear Heqincrement.
+
+assert (LocalVarsUndeclare: forall l40 l50 vc,
+  LocalVarsAgree l40 l50 vc
+   ->
+  LocalVarsAgree l40 (map_remove (map_remove l50
+                                             (cursor_name loop_depth))
+                                 (offset_name loop_depth))
+                 vc).
+{
+  intros l40 l50 vc LVA k L.
+  rewrite<- (LVA k L).
+  unfold map_remove. unfold map_lookup.
+  repeat rewrite Map.remove_ok.
+  repeat rewrite Map.insert_ok.
+  subst offset_name cursor_name.
+  destruct string_dec. { discriminate. }
+  destruct string_dec. { discriminate. }
+  trivial.
+}
+
+assert (StmtResultsUndeclare: forall w40 w50 l40 l50 r40 r50 vc,
+  StmtResultsAgree (w40, l40, r40) (w50, l50, r50) vc
+   ->
+  StmtResultsAgree (w40, l40, r40)
+                   (w50,
+                    map_remove (map_remove l50
+                                           (cursor_name loop_depth))
+                               (offset_name loop_depth),
+                    r50) vc).
+{
+  unfold StmtResultsAgree.
+  intros w40 w50 l40 l50 r40 r50 vc SRA.
+  destruct SRA as (LVA, SRA). split. { apply (LocalVarsUndeclare l40 l50 vc LVA). }
+  assumption.
+}
+
+assert (UndeclareSV: forall ctx l,
+  SecondaryVarsOk (ctx :: loop_info) l
+   ->
+  SecondaryVarsOk loop_info (map_remove (map_remove l
+                                                    (cursor_name loop_depth))
+                                        (offset_name loop_depth))).
+{
+  intros ctx l SV'.
+  unfold map_remove.
+  split; unfold LoopOffsetsAgree; unfold LoopCursorsAgree; unfold map_lookup;
+         repeat rewrite Map.remove_ok;
+         repeat rewrite Map.insert_ok;
+         try rewrite Heqoffset_name; try rewrite Heqcursor_name.
+  { apply (sv_result_declared SV'). }
+  {
+    intros k L.
+    assert (LO := sv_offsets_agree SV' k (Nat.lt_lt_succ_r _ _ L)). unfold LoopOffsetsAgree in LO.
+    unfold map_lookup in LO.
+    repeat rewrite Map.remove_ok.
+    destruct string_dec as [E|]. { apply make_var_name_inj in E. lia. }
+    destruct string_dec. { discriminate. }
+    rewrite<- Heqoffset_name in LO. cbn in LO.
+    replace (Datatypes.length loop_info - 0 - k) with (S (Datatypes.length loop_info - 1 - k))
+      in LO by lia.
+    cbn in LO. subst offset_name.
+    apply LO; assumption.
+  }
+  {
+    intros k L.
+    assert (LC := sv_cursors_agree SV' k (Nat.lt_lt_succ_r _ _ L)). unfold LoopOffsetsAgree in LC.
+    unfold map_lookup in LC.
+    repeat rewrite Map.remove_ok.
+    destruct string_dec. { discriminate. }
+    destruct string_dec as [E|]. { apply make_var_name_inj in E. lia. }
+    rewrite<- Heqcursor_name in LC. cbn in LC.
+    replace (Datatypes.length loop_info - 0 - k) with (S (Datatypes.length loop_info - 1 - k))
+      in LC by lia.
+    cbn in LC. subst cursor_name.
+    apply LC; assumption.
+  }
+  {
+    intros k L. repeat rewrite Map.remove_ok.
+    destruct string_dec. { trivial. }
+    destruct string_dec. { discriminate. }
+    apply le_lt_or_eq in L.
+    destruct L as [L|E]. { apply (sv_offsets_undeclared SV' k L). }
+    assert (K: loop_depth = N.of_nat k) by lia.
+    subst loop_depth. contradiction.
+  }
+  {
+    intros k L. repeat rewrite Map.remove_ok.
+    destruct string_dec. { discriminate. }
+    destruct string_dec. { trivial. }
+    apply le_lt_or_eq in L.
+    destruct L as [L|E]. { apply (sv_cursors_undeclared SV' k L). }
+    assert (K: loop_depth = N.of_nat k) by lia.
+    subst loop_depth. contradiction.
+  }
+}
+
+(* check the special zero loop case *)
+remember (Z.to_nat (Z_of_uint256 count)) as c.
+destruct c.
+{ (* count = 0 *)
+  subst iterate40.
+  assert (W: iterate50 max_loop_iterations world current_loc50 
+              =
+             (world, current_loc50, Some StmtSuccess)).
+  {
+    subst iterate50.
+    destruct max_loop_iterations. { now apply N.nlt_0_r in EnoughIterations. }
+    cbn. unfold map_lookup in *. rewrite CondExprWorks with (cursor := zero256).
+    {
+      replace (Z_of_uint256 zero256 <? Z_of_uint256 count)%Z with false.
+      { cbn. unfold zero256. rewrite uint256_ok. easy. }
+      unfold zero256. rewrite uint256_ok.
+      rewrite<- (Z2Nat.id (Z_of_uint256 count)). { now rewrite<- Heqc. }
+      apply (proj1 (uint256_range count)).
+    }
+    subst current_loc50. rewrite Map.insert_ok.
+    destruct string_dec as [|NE]. 2:{ contradiction. }
+    unfold int_zero_value. unfold yul_uint256.
+    repeat f_equal.
+    apply Eqdep_dec.eq_proofs_unicity.
+    decide equality.
+  }
+  rewrite W.
+
+  split.
+  {
+    cbn. split. 2:trivial.
+    apply LocalVarsUndeclare. assumption.
+  }
+  subst current_loc50.
+  split; unfold LoopOffsetsAgree; unfold LoopCursorsAgree; unfold map_lookup; unfold map_remove; intros;
+         repeat rewrite Map.remove_ok;
+         repeat rewrite Map.insert_ok;
+         subst offset_name cursor_name.
+  {
+    destruct string_dec. { discriminate. }
+    destruct string_dec. { discriminate. }
+    apply (sv_result_declared SV).
+  }
+  {
+    assert (LO := sv_offsets_agree SV). unfold LoopOffsetsAgree in LO. 
+    unfold map_lookup in LO.
+    destruct string_dec as [E|]. { apply make_var_name_inj in E. lia. }
+    destruct string_dec. { discriminate. }
+    apply LO; assumption.
+  }
+  {
+    assert (LC := sv_cursors_agree SV). unfold LoopCursorsAgree in LC. 
+    unfold map_lookup in LC.
+    destruct string_dec. { discriminate. }
+    destruct string_dec as [E|]. { apply make_var_name_inj in E. lia. }
+    apply LC; assumption.
+  }
+  {
+    destruct string_dec. { trivial. }
+    destruct string_dec. { discriminate. }
+    apply (sv_offsets_undeclared SV); assumption.
+  }
+  {
+    destruct string_dec. { discriminate. }
+    destruct string_dec. { trivial. }
+    apply (sv_cursors_undeclared SV); assumption.
+  }
+}
+(* now c = count - 1 and we can form a context *)
+pose (current_ctx := {| L40.Expr.loop_offset := let _ := memory_impl in OpenArray.get loc40 var
+                      ; L40.Expr.loop_count := count
+                      ; L40.Expr.loop_countdown := c
+                     |}).
+cbn in current_ctx.
+assert (PreloopSV: SecondaryVarsOk (current_ctx :: loop_info) current_loc50).
+{
+  subst current_loc50.
+  split; unfold map_lookup.
+  {
+    repeat rewrite Map.insert_ok. subst offset_name cursor_name.
+    destruct string_dec. { discriminate. }
+    destruct string_dec. { discriminate. }
+    apply (sv_result_declared SV).
+  }
+  {
+    intros k L. rewrite<- Heqoffset_name. cbn.
+    rewrite Nat.sub_0_r.
+    remember (Datatypes.length loop_info - k) as i.
+    cbn in L. destruct i; cbn.
+    {
+      assert (K: k = List.length loop_info) by lia.
+      unfold map_lookup. repeat rewrite Map.insert_ok.
+      subst offset_name cursor_name.
+      destruct string_dec. { discriminate. }
+      destruct string_dec. { trivial. }
+      subst k. rewrite LoopDepthOk in *.
+      rewrite N2Nat.id in *. contradiction.
+    }
+    assert (L': k < Datatypes.length loop_info) by lia.
+    assert (A := sv_offsets_agree SV k L').
+    replace i with (Datatypes.length loop_info - 1 - k) by lia.
+    subst offset_name.
+    unfold map_lookup in *. repeat rewrite Map.insert_ok.
+    destruct string_dec. { subst. discriminate. }
+    destruct string_dec as [E|]. { apply make_var_name_inj in E. lia. }
+    apply A.
+  }
+  {
+    intros k L. rewrite<- Heqcursor_name. cbn.
+    rewrite Nat.sub_0_r.
+    remember (Datatypes.length loop_info - k) as i.
+    cbn in L. destruct i; cbn.
+    {
+      assert (K: k = List.length loop_info) by lia.
+      unfold map_lookup. repeat rewrite Map.insert_ok.
+      subst offset_name cursor_name.
+      destruct string_dec.
+      {
+        subst current_ctx. unfold get_cursor. cbn.
+        replace (Z_of_uint256 count - 1 - Z.of_nat c)%Z with 0%Z by lia.
+        repeat f_equal. unfold int_zero_value. unfold yul_uint256. unfold zero256.
+        f_equal. apply eq_proofs_unicity. decide equality.
+      }
+      destruct string_dec. { discriminate. }
+      subst k. rewrite LoopDepthOk in *.
+      rewrite N2Nat.id in *. contradiction.
+    }
+    assert (L': k < Datatypes.length loop_info) by lia.
+    assert (A := sv_cursors_agree SV k L').
+    replace i with (Datatypes.length loop_info - 1 - k) by lia.
+    subst cursor_name.
+    unfold map_lookup in *. repeat rewrite Map.insert_ok.
+    destruct string_dec as [E|]. { apply make_var_name_inj in E. lia. }
+    destruct string_dec. { subst. discriminate. }
+    apply A.
+  }
+  {
+    intros k Bound. cbn in Bound.
+    repeat rewrite Map.insert_ok.
+    subst offset_name cursor_name.
+    destruct string_dec. { discriminate. }
+    destruct string_dec as [E|]. { apply make_var_name_inj in E. lia. }
+    apply (sv_offsets_undeclared SV k). lia.
+  }
+  intros k Bound. cbn in Bound.
+  repeat rewrite Map.insert_ok.
+  subst offset_name cursor_name.
+  destruct string_dec as [E|]. { apply make_var_name_inj in E. lia. }
+  destruct string_dec. { discriminate. }
+  apply (sv_cursors_undeclared SV k). lia.
+}
+
+assert (G: forall ctx l,
+             LoopCursorsAgree (ctx :: loop_info) l
+              ->
+             map_lookup l (cursor_name loop_depth)
+              =
+             Some (existT _ U256 (yul_uint256 (get_cursor ctx)))).
+{
+  intros ctx l LCA.
+  assert (L := LCA (List.length loop_info) (Nat.lt_succ_diag_r _)).
+  rewrite<- Heqcursor_name in L.
+  cbn in L.
+  rewrite Nat.sub_0_r in L.
+  rewrite Nat.sub_diag in L.
+  cbn in L. rewrite LoopDepthOk in L.
+  rewrite N2Nat.id in L.
+  exact L.
+}
+
+assert (IncrementSV: forall offset l m,
+                       let ctx := {| L40.Expr.loop_offset := offset
+                                   ; L40.Expr.loop_count := count
+                                   ; L40.Expr.loop_countdown := S m
+                                  |} in
+                       (Z.of_nat (S m) < Z_of_uint256 count)%Z
+                        ->
+                       SecondaryVarsOk (ctx :: loop_info) l
+                        ->
+                       SecondaryVarsOk
+                         ({| L40.Expr.loop_offset := offset
+                           ; L40.Expr.loop_count := count
+                           ; L40.Expr.loop_countdown := m
+                          |} :: loop_info)
+                          (map_insert l (cursor_name loop_depth)
+                             (existT _ U256 (yul_uint256
+                                              (uint256_of_Z (Z_of_uint256 (get_cursor ctx) + 1%Z)))))).
+{
+  cbn.
+  intros offset l m Bound SV'.
+  split; unfold map_lookup in *; unfold map_insert in *; unfold map_remove in *;
+    repeat rewrite Map.insert_ok.
+  {
+    subst offset_name cursor_name.
+    destruct string_dec. { discriminate. }
+    apply (sv_result_declared SV').
+  }
+  {
+    intros k L. rewrite<- Heqoffset_name. cbn.
+    unfold map_insert. unfold map_lookup. rewrite Map.insert_ok.
+    destruct string_dec. { subst. discriminate. }
+    assert (X := sv_offsets_agree SV' k L).
+    subst. apply X.
+  }
+  {
+    intros k L. rewrite<- Heqcursor_name. cbn.
+    unfold map_insert. unfold map_lookup. rewrite Map.insert_ok.
+    destruct string_dec as [E|NE].
+    {
+      subst. apply make_var_name_inj in E. subst loop_depth.
+      rewrite Nat2N.id in LoopDepthOk. subst k.
+      rewrite Nat.sub_0_r.
+      rewrite Nat.sub_diag.
+      cbn.
+      unfold get_cursor. cbn.
+      f_equal. f_equal. f_equal. f_equal.
+      rewrite uint256_ok.
+      replace (((Z_of_uint256 count - 1 - Z.pos (Pos.of_succ_nat m))) + 1)%Z
+        with (Z_of_uint256 count - 1 - Z.of_nat m)%Z
+        by lia.
+      assert (R := uint256_range count).
+      rewrite Z.mod_small; lia.
+    }
+    assert (X := sv_cursors_agree SV' k L).
+    rewrite<- Heqcursor_name in X. cbn in X.
+    remember (Datatypes.length loop_info - 0 - k) as i.
+    destruct i.
+    {
+      cbn in L.
+      now replace loop_depth with (N.of_nat k) in NE by lia.
+    }
+    cbn.
+    apply X.
+  }
+  {
+    intros k L.
+    rewrite Map.insert_ok. subst cursor_name.
+    destruct string_dec. { discriminate. }
+    apply (sv_offsets_undeclared SV' k L).
+  }
+  intros k L.
+  rewrite Map.insert_ok. subst offset_name.
+  destruct string_dec as [E|NE].
+  {
+    subst cursor_name. apply make_var_name_inj in E.
+    cbn in L. lia.
+  }
+  apply (sv_cursors_undeclared SV' k L).
+}
+
+assert (EnoughIterationsForBody: (AST.max_loop_count_block bodyblock40 
+                                   <
+                                  N.of_nat max_loop_iterations)%N).
+{ subst. cbn. apply (max_lub_lt_r EnoughIterations). }
+subst bodyblock40 bodyblock50.
+assert (T: translate_block match this_fun_decl50 with
+           | Some _ => true
+           | None => false
+           end B protos (L40.AST.Block body) (N.succ loop_depth) = inr (AST.Block body50)).
+{ cbn. now rewrite<- Heqbody'. }
+
+(* ------------------------------- induction ---------------------------- *)
+clear Heqcurrent_loc50.
+remember (S c) as sc.
+assert (CBound: (Z.of_nat c < Z_of_uint256 count)%Z) by lia.
+assert (M: sc < max_loop_iterations) by lia.
+clear Heqc.
+unfold current_ctx in *.
+assert (CurrentSV: match sc with
+                   | O => True
+                   | S x => SecondaryVarsOk ({|
+                                              Expr.loop_offset := let _ := memory_impl in
+                                                                  OpenArray.get loc40 var;
+                                              Expr.loop_count := count;
+                                              Expr.loop_countdown := x
+                                             |} :: loop_info) current_loc50
+                   end).
+{
+  subst sc.
+  apply PreloopSV.
+}
+clear PreloopSV.
+clear LocalVarsOk.
+remember (_ loc40 var) as offset. clear Heqoffset.
+revert loc40 c CBound Heqsc current_ctx current_loc50 CurrentSV CurrentLocalVarsOk world.
+remember max_loop_iterations as fixed_max_loop_iterations.
+rewrite Heqfixed_max_loop_iterations in M.
+rewrite Heqfixed_max_loop_iterations. clear Heqfixed_max_loop_iterations.
+revert max_loop_iterations M.
+induction sc; intros. { discriminate. }
+inversion Heqsc; subst sc; clear Heqsc.
+
+assert (LoopDepthOk': List.length (current_ctx :: loop_info) = N.to_nat (N.succ loop_depth)).
+{ cbn. rewrite LoopDepthOk. lia. }
+assert (BodyWorks := interpret_translated_block_weak call40 call50 CallsOk decls40 decls50
+                                                     this_fun_decl40 this_fun_decl50 FunDeclOk
+                                                     DeclsOk builtins40 builtins50 BuiltinsOk
+                                                     BuiltinsBasics BuiltinsSafe ProtosOk
+                                                     world loc40 current_loc50
+                                                     (current_ctx :: loop_info) LoopDepthOk' CurrentSV
+                                                     (L40.AST.Block body) (L50.AST.Block body50)
+                                                     T varcap (N.max_lub_r _ _ _ VarcapOk)
+                                                     CurrentLocalVarsOk EnoughIterationsForBody
+                                                     H).
+
+subst iterate40 iterate50.
+fold current_ctx.
+
+destruct max_loop_iterations. { exfalso. apply (Nat.nlt_0_r _ M). }
+cbn.
+assert (CondRewrite := CondExprWorks world current_loc50 (get_cursor current_ctx)
+                                     (G current_ctx current_loc50 (sv_cursors_agree CurrentSV))).
+unfold map_lookup in CondRewrite. rewrite CondRewrite. clear CondRewrite.
+assert (ShouldProceed: (Z_of_uint256 (get_cursor current_ctx) <? Z_of_uint256 count)%Z = true).
+{
+  apply Z.ltb_lt.
+  unfold get_cursor.
+  unfold current_ctx.
+  cbn.
+  rewrite uint256_ok. 
+  assert (R := uint256_range count).
+  rewrite Z.mod_small; lia.
+}
+rewrite ShouldProceed. unfold one256. cbn. rewrite uint256_ok. cbn.
+cbn in BodyWorks.
+rewrite<- interpret_stmt_list_ok in BodyWorks.
+cbn in BodyWorks.
+destruct (_ world current_loc50 body50) as ((world50', loc50'), result50').
+destruct (_ world loc40 (current_ctx :: loop_info) body) as ((world40', loc40'), result40').
+destruct BodyWorks as (PostIterResultsAgree, PostIterSV).
+unfold StmtResultsAgree in PostIterResultsAgree.
+destruct PostIterResultsAgree as (PostIterLocalVarsOk, PostIterResultsAgree).
+
+(* apply increment *)
+assert (IncRewrite := IncrementWorks world50' loc50' (get_cursor current_ctx)
+                                     (G current_ctx loc50' (sv_cursors_agree PostIterSV))).
+unfold map_lookup in IncRewrite. rewrite IncRewrite. clear IncRewrite.
+remember (map_insert loc50' (cursor_name loop_depth)
+           (existT (fun t : yul_type => yul_value t) U256
+              (yul_uint256 (uint256_of_Z (Z_of_uint256 (get_cursor current_ctx) + 1)))))
+  as postinc_loc50.
+assert (NextSV:
+     match c with
+     | 0 => True
+     | S x =>
+         SecondaryVarsOk
+           ({|
+              Expr.loop_offset := offset;
+              Expr.loop_count := count;
+              Expr.loop_countdown := x
+            |} :: loop_info) postinc_loc50
+     end).
+{
+  destruct c as [|x]. { trivial. }
+  cbn. subst postinc_loc50.
+  apply (IncrementSV _ loc50' x CBound PostIterSV).
+}
+assert (StopNowSV := UndeclareSV current_ctx loc50' PostIterSV).
+destruct result40' as [result40'|], result50' as [result50'|]; try contradiction.
+2:{
+  (* just undeclare the offset and cursor *)
+  split. { apply StmtResultsUndeclare. cbn. tauto. }
+  apply StopNowSV.
+}
+
+assert (EquivSV: forall ctx loc1 loc2,
+                   (forall name, map_lookup loc1 name = map_lookup loc2 name)
+                    ->
+                   SecondaryVarsOk ctx loc1
+                    ->
+                   SecondaryVarsOk ctx loc2).
+{
+  intros ctx loc1 loc2 E SV1.
+  split.
+  { rewrite<- E. apply (sv_result_declared SV1). }
+  { intros k L. rewrite<- E. apply (sv_offsets_agree SV1 k L). }
+  { intros k L. rewrite<- E. apply (sv_cursors_agree SV1 k L). }
+  { intros k L. rewrite<- E. apply (sv_offsets_undeclared SV1 k L). }
+  intros k L. rewrite<- E. apply (sv_cursors_undeclared SV1 k L).
+}
+
+assert (StopNowSV':
+  SecondaryVarsOk loop_info
+    (map_remove
+       (map_remove
+          (map_insert loc50' (cursor_name loop_depth)
+             (existT (fun t : yul_type => yul_value t) U256
+                (yul_uint256 (uint256_of_Z (Z_of_uint256 (uint256_of_Z (Z_of_uint256 count - 1 - 0)) + 1)))))
+          (cursor_name loop_depth)) (offset_name loop_depth))).
+{
+  refine (EquivSV _ _ _ _ StopNowSV).
+  intro name. unfold map_lookup; unfold map_remove; unfold map_insert.
+  repeat rewrite Map.remove_ok. repeat rewrite Map.insert_ok.
+  destruct string_dec; try easy; destruct string_dec; easy.
+}
+
+assert (StopNowLVA:
+  LocalVarsAgree loc40' (map_remove (map_remove loc50' (cursor_name loop_depth)) (offset_name loop_depth))
+    varcap).
+{ now apply LocalVarsUndeclare. }
+
+assert (StopNowLVA':
+  LocalVarsAgree loc40'
+    (map_remove
+       (map_remove
+          (map_insert loc50' (cursor_name loop_depth)
+             (existT (fun t : yul_type => yul_value t) U256
+                (yul_uint256 (uint256_of_Z (Z_of_uint256 (uint256_of_Z (Z_of_uint256 count - 1 - 0)) + 1)))))
+          (cursor_name loop_depth)) (offset_name loop_depth)) varcap).
+{
+  apply LocalVarsUndeclare.
+  intros k L. unfold map_insert. unfold map_lookup. rewrite Map.insert_ok.
+  subst cursor_name. destruct string_dec. { discriminate. }
+  apply (PostIterLocalVarsOk k L).
+}
+
+destruct c as [|c'].
+{
+  (* we finish it *)
+  cbn.
+  destruct max_loop_iterations. { lia. } (* we pay for a whole iteration just to check the condition! *)
+  cbn.
+  assert (PostincCursor: map_lookup postinc_loc50 (cursor_name loop_depth) 
+              =
+             Some
+               (existT (fun t : yul_type => yul_value t) U256
+                  (yul_uint256 (uint256_of_Z (Z_of_uint256 (get_cursor current_ctx) + 1))))).
+  {
+    unfold map_lookup. subst postinc_loc50. unfold map_insert.
+    rewrite Map.insert_ok. now destruct string_dec.
+  }
+
+  assert (CondRewrite := CondExprWorks world50' postinc_loc50 
+                                       (uint256_of_Z (Z_of_uint256 (get_cursor current_ctx) + 1))
+                                       PostincCursor).
+  unfold map_lookup in CondRewrite.
+  subst postinc_loc50.
+  unfold dynamic_value in CondRewrite.
+  rewrite CondRewrite. clear CondRewrite.
+
+  unfold current_ctx. unfold get_cursor. cbn.
+  replace (Z_of_uint256
+                 (uint256_of_Z (Z_of_uint256 (uint256_of_Z (Z_of_uint256 count - 1 - 0)) + 1)))%Z
+    with (Z_of_uint256 count).
+  2:{
+    assert (R := uint256_range count).
+    repeat rewrite uint256_ok.
+    rewrite Z.mod_small; rewrite Z.mod_small; lia.
+  }
+  replace (Z_of_uint256 count <? Z_of_uint256 count)%Z with false.
+  2:{ symmetry. apply Z.ltb_ge. lia. }
+  unfold zero256. cbn. rewrite uint256_ok. cbn.
+  destruct result40' as [|a40|x40], result50' as [|a50|x50]; try destruct a40; try destruct a50;
+    try easy; split; try assumption; split; assumption.
+} (* c = 0 *)
+
+assert (C'Bound: (Z.of_nat c' < Z_of_uint256 count)%Z) by lia.
+assert (PostIncLVA: LocalVarsAgree loc40' postinc_loc50 varcap).
+{
+  intros k L. unfold map_lookup. subst postinc_loc50. unfold map_insert. 
+  rewrite Map.insert_ok.
+  subst. destruct string_dec; try discriminate.
+  apply (PostIterLocalVarsOk k L).
+}
+assert (IH := IHsc max_loop_iterations (lt_S_n _ _ M)
+              loc40' c' C'Bound eq_refl postinc_loc50 NextSV PostIncLVA world50'). clear IHsc.
+cbn.
+cbn in IH.
+unfold dynamic_value in *.
+subst postinc_loc50.
+remember (fix interpret_stmt_list_metered
+            (world0 : world_state) (loc : memory) (loops : list Expr.loop_ctx) (l0 : list L40.AST.stmt)
+            {struct l0} : world_state * memory * option (stmt_result uint256) := _)
+  as interpret_stmt_list40.
+remember (fix do_loop (world0 : world_state) (loc : memory) (countdown : nat) {struct countdown} :
+               world_state * memory * option (stmt_result uint256) := _) as iterate40.
+remember (fix iterate
+              (count0 : nat) (world0 : world_state) (loc : string_map {t : yul_type & yul_value t})
+              {struct count0} :
+                world_state * string_map {t : yul_type & yul_value t} *
+                option (stmt_result (list {t : yul_type & yul_value t})) := _) as iterate50.
+
+destruct result40' as [|a40|x40], result50' as [|a50|x50]; try contradiction;
+  try destruct a40; try destruct a50; try easy;
+  try subst world40'; try apply IH.
+Qed.
