haskell/BuiltinsParser.y
@@ -1,0 +1,44 @@
+{
+module BuiltinsParser where
+
+import PatchedExtracted hiding (map, div, Int)
+import qualified Token
+import qualified Data.Text
+import Data.Text.Encoding (encodeUtf8)
+import qualified Data.ByteString
+}
+
+%name parse
+%tokentype { Token.Token }
+%error { parseError }
+
+%token
+    name   { Token.Name $$ }
+    newline { Token.Newline }
+
+    '('  { Token.OpenParen }
+    ')'  { Token.CloseParen }
+    ','  { Token.Comma }
+    "->"  { Token.Arrow }
+
+%%
+
+All : Proto     { [$1] }
+    | Proto All { $1 : $2 }
+    | newline All { $2 }
+
+Proto : name Args "->" Types newline { Build_proto_ast $1 $2 $4 } 
+      | name Args            newline { Build_proto_ast $1 $2 [] }
+
+Args : '(' ')'       { [] }
+     | '(' Types ')' { $2 }
+
+Types : name           { [$1] }
+      | name ',' Types { $1 : $3 }
+
+{
+parseError :: [Token.Token] -> a
+parseError ts = error $ "Parse error: " ++ show (take 10 ts)
+}
+
+-- vim: set ft=haskell:
